 @prefix qgiscf: <https://linked.data.gov.au/def/qg-security-classifications/> .

 @prefix dc: <http://purl.org/dc/elements/1.1/> .
 @prefix dcterms: <http://purl.org/dc/terms/> .
 @prefix rdf: <http://www.w3.org/1999/02/22-rdf-syntax-ns#> .
 @prefix rdfs: <http://www.w3.org/2000/01/rdf-schema#> .
 @prefix skos: <http://www.w3.org/2004/02/skos/core#> .
 @prefix xsd: <http://www.w3.org/2001/XMLSchema#> .
 @prefix sdo: <http://www.schema.org/> .
 @prefix owl: <http://www.w3.org/2002/07/owl#> .

<https://linked.data.gov.au/def/qg-security-classifications> a owl:Ontology , skos:ConceptScheme ;
dcterms:created "2020-11-11"^^xsd:date ;
dcterms:creator <https://linked.data.gov.au/def/gsq-alias/des> ;
dcterms:modified "2022-03-25"^^xsd:date ;
dcterms:publisher <https://linked.data.gov.au/def/gsq-alias/des> ;
dcterms:provenance "Queensland Government Information Security Policy (IS18:2018) and the Queensland Government Information Security Classification Framework (QGSCIF)"@en ;
skos:definition "This is a vocabulary collection used by the Queensland Government to determine the security classifications for the dataset.  It is used by the dataset classification and access restrictions property."@en ;
skos:prefLabel "Queensland Government Information Security Classifications"@en ;
skos:hasTopConcept 
    qgiscf:official ,
    qgiscf:sensitive  ,
    qgiscf:protected .

<https://linked.data.gov.au/def/gsq-alias/des>
    a sdo:Organization ;
    sdo:name "Department of Environment and Science"@en .

qgiscf:official a skos:Concept ; 
 skos:topConceptOf <https://linked.data.gov.au/def/qg-security-classifications> ; 
 skos:definition "OFFICIAL represents most Queensland Government information by volume, but lowest business impact per document if compromised or lost. However, where information is aggregated on an information asset such as an ICT server, the impact of compromise may increase and with it, the controls.  OFFICIAL information is routine information without special sensitivity or handling requirements. All routine public-sector business, operations and services is treated as OFFICIAL. At the OFFICIAL classification there is a general presumption that data may be shared across government. Security measures should be proportionate and driven by the business requirement.  Most OFFICIAL information is subject to the Public Records Act 2002 (Qld)."@en ;
 skos:inScheme <https://linked.data.gov.au/def/qg-security-classifications> ;
 skos:notation "off" ;
 rdfs:label "OFFICIAL"@en ;
 skos:prefLabel "OFFICIAL"@en  .

qgiscf:official-public a skos:Concept ; 
 skos:broader qgiscf:official ;
 skos:definition "As per OFFICIAL with the Dissemination Limiting Marking (DLM) applied to indicates the information is publically available and may be accessed by or released to the public."@en ;
 skos:inScheme <https://linked.data.gov.au/def/qg-security-classifications> ;
 skos:notation "ofp" ;
 skos:prefLabel "OFFICIAL-PUBLIC"@en  .

qgiscf:sensitive a skos:Concept ;  
 skos:topConceptOf <https://linked.data.gov.au/def/qg-security-classifications> ; 
 skos:definition "The use of the SENSITIVE indicates that information requires additional handling care due to its sensitivity or moderate business impact if compromised or lost.  SENSITIVE information must be labelled.  Examples of SENSITIVE information may include: government or agency business, whose compromise could affect the government's capacity to make decisions or operate, the public's confidence in government, the stability of the market place and so on commercial interests, whose compromise could significantly affect the competitive process and provide the opportunity for unfair advantage legal professional privilege law enforcement operations whose compromise could adversely affect crime prevention strategies, particular investigations or adversely affect personal safety personal information, which is required to be safeguarded under the Information Privacy Act 2009 (Qld), or other legislation."@en ;
 skos:inScheme <https://linked.data.gov.au/def/qg-security-classifications> ;
 skos:notation "sns" ;
 skos:prefLabel "SENSITIVE"@en  .

qgiscf:protected a skos:Concept ;
 skos:topConceptOf <https://linked.data.gov.au/def/qg-security-classifications> ;
 skos:definition "PROTECTED information requires the most careful safeguards due to its sensitivity or major business impact if compromised or lost. PROTECTED information assets require a substantial degree of control as compromise could cause serious damage to the State, the Government, commercial entities or members of the public. PROTECTED information must be labelled. Cabinet information is PROTECTED. Cabinet documents (CABINET information) can be damaging to the public policy agenda and the government generally, and to the public interest. Unlawful disclosure of Cabinet information may constitute an offence under the Criminal Code Act 1899 (Qld), Public Sector Ethics Act 1994 (Qld) and may constitute official misconduct under the Crime and Misconduct Act 2001 (Qld). The primary guidance document to support these processes, including the handling of Cabinet material, is the Queensland Cabinet Handbook. Most PROTECTED information is subject the Public Records Act 2002 (Qld)."@en ;
 skos:inScheme <https://linked.data.gov.au/def/qg-security-classifications> ;
 skos:notation "prtc" ;
 skos:prefLabel "PROTECTED"@en  .

qgiscf:qesd-qgiscf a skos:Collection  ;
 skos:prefLabel "QESD QGISCF"@en ;
 rdfs:label "Queensland Environemnt Science Data collection of the Qld Gov Information Security Classification"@en ;
 skos:definition "Collection of terms used for the QESD Catalogue from the QGISCF vocabulary for the standard terms in the framework."@en ;
 skos:member 
    qgiscf:official , 
    qgiscf:official-public ,
    qgiscf:sensitive  ,
    qgiscf:protected .
