@prefix dc: <http://purl.org/dc/elements/1.1/> .
@prefix dcterms: <http://purl.org/dc/terms/> .
@prefix gsqst: <http://linked.data.gov.au/def/geological-sites/> .
@prefix owl: <http://www.w3.org/2002/07/owl#> .
@prefix rdf: <http://www.w3.org/1999/02/22-rdf-syntax-ns#> .
@prefix rdfs: <http://www.w3.org/2000/01/rdf-schema#> .
@prefix sdo: <http://schema.org/> .
@prefix skos: <http://www.w3.org/2004/02/skos/core#> .
@prefix xsd: <http://www.w3.org/2001/XMLSchema#> .

<http://linked.data.gov.au/def/geological-sites> a owl:Ontology ,
        skos:ConceptScheme ;
    dcterms:created "2020-02-07"^^xsd:date ;
    dcterms:creator <http://linked.data.gov.au/org/gsq> ;
    dcterms:modified "2022-04-19"^^xsd:date ;
    dcterms:publisher <http://linked.data.gov.au/org/gsq> ;
    dcterms:provenance "Compiled by the Geological Survey of Queensland" ;
    skos:definition "The proximate geological features and locations that may be sampled or observed to determine the geological properties of an ultimate feature of interest."@en ;
    skos:hasTopConcept 
        gsqst:auger,
        gsqst:base-station,
        gsqst:borehole,
        gsqst:cutting,
        gsqst:field-site,
        gsqst:mine,
        gsqst:pit,
        gsqst:project-site,
        gsqst:quarry,
        gsqst:geofeature,
        gsqst:trench,
        gsqst:administrative-area,
        #gsqst:wellbore,
        gsqst:unknown ;
    skos:prefLabel "Geological Sites"@en .

<http://linked.data.gov.au/org/gsq> a sdo:Organization ;
    sdo:name "Geological Survey of Queensland" ;
    sdo:url "http://www.business.qld.gov.au/industries/mining-energy-water/resources/geoscience-information/gsq"^^xsd:anyURI .

gsqst:auger a skos:Concept ;
    skos:altLabel "Auger Hole"@en ;
    skos:definition "A shallow drill hole conducted for the purpose of extraction of soil or rock samples. Sources: GSQ."@en ;
    skos:scopeNote "In the context of administration by a regulatory body, a borehole exists as an entity once proposed-to-be-drilled, prior to drilling and having a tangible physical manifestation."@en ;
    rdfs:isDefinedBy <http://linked.data.gov.au/def/geological-sites> ;
    skos:inScheme <http://linked.data.gov.au/def/geological-sites> ;
    skos:notation "au" ;
    skos:prefLabel "Auger"@en ;
    skos:topConceptOf <http://linked.data.gov.au/def/geological-sites> .

gsqst:base-station a skos:Concept ;
    skos:definition "A site of known location for the samplng or measurement of a property or as a point with a known measurement of a property for the calibration of a larger survey."@en ;
    rdfs:isDefinedBy <http://linked.data.gov.au/def/geological-sites> ;
    skos:inScheme <http://linked.data.gov.au/def/geological-sites> ;
    skos:notation "bs" ;
    skos:prefLabel "Base Station"@en ;
    skos:topConceptOf <http://linked.data.gov.au/def/geological-sites> .

gsqst:borehole a skos:Concept ;
    skos:altLabel "Bore"@en,
        "Core Hole"@en,
        "Corehole"@en,
        "Drillhole"@en,
        "Well"@en ;
    skos:definition "A Borehole is a deep and narrow hole in the ground typically made by a drilling rig. Boreholes are the sites of extraction of rock samples, such as core, cuttings, and rock chips, and fluid samples. They may be designed primarily to extract rock or fluid samples, to exchange (or facilitate the exchange of) fluids between a subsurface reservoir and the surface (or another reservoir), or to enable the detection and measurement of rock or fluid properties. A Borehole has a single Origin and all Wellbore(s) that extend from this Well Origin are parts of the Borehole. The term borehole is generic and has variations in terminology that are industry and location specific. Some industries and locations may not recognise the term borehole as a standard designation. Sources: PPDM What Is A Well, GSQ."@en ;
    skos:scopeNote "In the context of administration by a regulatory body, a borehole exists as an entity once proposed-to-be-drilled and prior to physical creation through the act of drilling."@en ;
    rdfs:isDefinedBy <http://linked.data.gov.au/def/geological-sites> ;
    skos:inScheme <http://linked.data.gov.au/def/geological-sites> ;
    skos:notation "bh" ;
    skos:prefLabel "Borehole"@en ;
    skos:topConceptOf <http://linked.data.gov.au/def/geological-sites> .

gsqst:cutting a skos:Concept ;
    skos:altLabel "Gutter"@en,
        "Road"@en,
        "Railway Cutting"@en,
        "Track"@en,
        "Tunnel"@en,
        "Drill Pad"@en ;
    skos:definition "A man-made excavation through the earth typically for infrastucture and/or transport."@en ;
    rdfs:isDefinedBy <http://linked.data.gov.au/def/geological-sites> ;
    skos:inScheme <http://linked.data.gov.au/def/geological-sites> ;
    skos:notation "ct" ;
    skos:prefLabel "Cutting"@en ;
    skos:scopeNote "A drill pad may be used where an at-surface sample or observation is taken at a drilling location. All sites where samples and observations made downhole are classified as boreholes."@en ;
    skos:topConceptOf <http://linked.data.gov.au/def/geological-sites> .

gsqst:field-site a skos:Concept ;
    skos:altLabel "Dig site"@en ;
    skos:definition "An area, transect, or point where samples are taken or observations are made directly from earth materials."@en ;
    rdfs:isDefinedBy <http://linked.data.gov.au/def/geological-sites> ;
    skos:inScheme <http://linked.data.gov.au/def/geological-sites> ;
    skos:notation "fs" ;
    skos:prefLabel "Field Site"@en ;
    skos:topConceptOf <http://linked.data.gov.au/def/geological-sites> .

gsqst:alluvial a skos:Concept ;
    skos:altLabel "Alluvium"@en ;
    skos:broader gsqst:field-site ;
    skos:definition "A field site from which a sediment sample transported by transport in a medium (air, water, ice) is taken or observation is made."@en ;
    rdfs:isDefinedBy <http://linked.data.gov.au/def/geological-sites> ;
    skos:inScheme <http://linked.data.gov.au/def/geological-sites> ;
    skos:notation "av" ;
    skos:prefLabel "Alluvial Site"@en .

gsqst:watercourse a skos:Concept ;
    skos:altLabel "Brook"@en,
        "Canal"@en,
        "Creek"@en,
        "Drain"@en,
        "River"@en,
        "Stream"@en ;
    skos:broader gsqst:alluvial ;
    skos:definition "The channel that a flowing body of water follows."@en ;
    rdfs:isDefinedBy <http://linked.data.gov.au/def/geological-sites> ;
    skos:inScheme <http://linked.data.gov.au/def/geological-sites> ;
    skos:notation "wc" ;
    skos:prefLabel "Watercourse"@en .
    
gsqst:beach a skos:Concept ;
    skos:altLabel "Shore"@en ;
    skos:broader gsqst:alluvial ;
    skos:definition "The land alongside a waterbody."@en ;
    rdfs:isDefinedBy <http://linked.data.gov.au/def/geological-sites> ;
    skos:inScheme <http://linked.data.gov.au/def/geological-sites> ;
    skos:notation "bc" ;
    skos:prefLabel "Beach"@en .

gsqst:waterbody a skos:Concept ;
    skos:altLabel "Dam"@en,
        "Dams"@en,
        "Lake"@en,
        "Pond"@en ;
    skos:broader gsqst:alluvial ;
    dcterms:provenance "Source: Merriam-Webster Dictionary" ;
    skos:definition "Any significant accumulation of typically non-flowing water, generally on a planet's surface. The term most often refers to oceans, seas, and lakes, but it includes smaller pools of water such as ponds, wetlands, or more rarely, puddles."@en ;
    rdfs:isDefinedBy <http://linked.data.gov.au/def/geological-sites> ;
    skos:inScheme <http://linked.data.gov.au/def/geological-sites> ;
    skos:notation "wy" ;
    skos:prefLabel "Waterbody"@en .

gsqst:colluvial a skos:Concept ;
    skos:altLabel "Boulders"@en,
        "Float"@en,
        "Roots"@en,
        "Rubble"@en,
        "Scree"@en,
        "Scree Slope"@en,
        "Talus"@en ;
    skos:broader gsqst:field-site ;
    skos:definition "A field site from which sediment is not primarily transported in a fluid, typically transported by gravity, where a sample is taken or observation is made. Bedrock is not exposed, but surface rock suggests bedrock is near surface."@en ;
    rdfs:isDefinedBy <http://linked.data.gov.au/def/geological-sites> ;
    skos:inScheme <http://linked.data.gov.au/def/geological-sites> ;
    skos:notation "cv" ;
    skos:prefLabel "Colluvial Site"@en .

gsqst:outcrop a skos:Concept ;
    skos:broader gsqst:field-site ;
    skos:definition "A field site where bedrock is exposed at the surface of the earth, and not concealed by regolith or water. There is a high degree of confidence that samples and observations from an outcrop site relate to the bedrock at that location."@en ;
    rdfs:isDefinedBy <http://linked.data.gov.au/def/geological-sites> ;
    skos:inScheme <http://linked.data.gov.au/def/geological-sites> ;
    skos:notation "oc" ;
    skos:prefLabel "Outcrop"@en .

gsqst:subcrop a skos:Concept ;
    skos:altLabel "sub-outcrop"@en ;
    skos:broader gsqst:outcrop ;
    skos:definition "A field site where bedrock is only exposed over a small area with very little topographic relief, to such an extent that the bedrock is reasonably inferred to be in-situ. There is a reasonable degree of confidence that samples and observations from a subcrop site relate to the bedrock at that location."@en ;
    rdfs:isDefinedBy <http://linked.data.gov.au/def/geological-sites> ;
    skos:inScheme <http://linked.data.gov.au/def/geological-sites> ;
    skos:notation "sc" ;
    skos:prefLabel "Subcrop"@en .

gsqst:regolith a skos:Concept ;
    skos:broader gsqst:field-site ;
    skos:definition "A field site at a layer of loose, heterogeneous superficial deposits covering solid rock."@en ;
    rdfs:isDefinedBy <http://linked.data.gov.au/def/geological-sites> ;
    skos:inScheme <http://linked.data.gov.au/def/geological-sites> ;
    skos:notation "rg" ;
    skos:prefLabel "Regolith"@en .

gsqst:pedolith a skos:Concept ;
    skos:altLabel "Soil"@en,
        "Soil Horizon"@en ;
    skos:broader gsqst:regolith ;
    skos:definition "A field site that has undergone pedogenic processes. Typically where a sample is taken or observation is made of soil."@en ;
    rdfs:isDefinedBy <http://linked.data.gov.au/def/geological-sites> ;
    skos:inScheme <http://linked.data.gov.au/def/geological-sites> ;
    skos:notation "pd" ;
    skos:prefLabel "Pedolith"@en .

gsqst:saprolith a skos:Concept ;
    skos:altLabel "Decomposed Granite"@en,
        "Decomposed Rock"@en,
        "Weathered Rock"@en,
        "Weathering Profile"@en ;
    skos:broader gsqst:regolith ;
    skos:definition "A field site from which a sample is taken or observation is made of chemically weathered rock ."@en ;
    rdfs:isDefinedBy <http://linked.data.gov.au/def/geological-sites> ;
    skos:inScheme <http://linked.data.gov.au/def/geological-sites> ;
    skos:notation "sr" ;
    skos:prefLabel "Saprolith"@en .

gsqst:tailings a skos:Concept ;
    skos:altLabel "Processing Plant"@en ;
    skos:broader gsqst:field-site ;
    skos:definition "An accumulation of material left over after the process of separating the valuable fraction from the uneconomic fraction (gangue) of an ore."@en ;
    rdfs:isDefinedBy <http://linked.data.gov.au/def/geological-sites> ;
    skos:inScheme <http://linked.data.gov.au/def/geological-sites> ;
    skos:notation "tl" ;
    skos:prefLabel "Tailings"@en .

gsqst:spoil a skos:Concept ;
    skos:altLabel "Mine Dump"@en,
        "Dump"@en,
        "Overburden"@en,
        "Interburden"@en,
        "Waste"@en ;
    skos:broader gsqst:field-site ;
    skos:definition "An accumulation of material removed to access an economically significant resource or ore body. Distinct from tailings, as spoil is physically removed from the ore prior to processing."@en ;
    rdfs:isDefinedBy <http://linked.data.gov.au/def/geological-sites> ;
    skos:inScheme <http://linked.data.gov.au/def/geological-sites> ;
    skos:notation "sl" ;
    skos:prefLabel "Spoil"@en .

gsqst:mine a skos:Concept ;
    dcterms:provenance "Source: Merriam-Webster Dictionary" ;
    skos:definition "A pit or excavation in the earth from which mineral substances are taken. Source: Merriam-Webster Dictionary"@en ;
    rdfs:isDefinedBy <http://linked.data.gov.au/def/geological-sites> ;
    skos:inScheme <http://linked.data.gov.au/def/geological-sites> ;
    skos:notation "mi" ;
    skos:prefLabel "Mine"@en ;
    skos:topConceptOf <http://linked.data.gov.au/def/geological-sites> .

gsqst:open-cut-mine a skos:Concept ;
    skos:broader gsqst:mine ;
    skos:definition "A pit or excavation in the earth, open to the ground surface, from which mineral substances are taken. Source: Merriam-Webster Dictionary"@en ;
    rdfs:isDefinedBy <http://linked.data.gov.au/def/geological-sites> ;
    skos:inScheme <http://linked.data.gov.au/def/geological-sites> ;
    skos:notation "om" ;
    skos:prefLabel "Open-Cut Mine"@en .

gsqst:underground-mine a skos:Concept ;
    skos:broader gsqst:mine ;
    skos:definition "An excavation in the earth, under the ground surface, from which mineral substances are taken. Source: Merriam-Webster Dictionary"@en ;
    rdfs:isDefinedBy <http://linked.data.gov.au/def/geological-sites> ;
    skos:inScheme <http://linked.data.gov.au/def/geological-sites> ;
    skos:notation "ug" ;
    skos:prefLabel "Underground Mine"@en .

gsqst:quarry a skos:Concept ;
    skos:definition "Man-made excavation to extract building and road base material."@en ;
    rdfs:isDefinedBy <http://linked.data.gov.au/def/geological-sites> ;
    skos:inScheme <http://linked.data.gov.au/def/geological-sites> ;
    skos:notation "qy" ;
    skos:prefLabel "Quarry"@en ;
    skos:topConceptOf <http://linked.data.gov.au/def/geological-sites> .

gsqst:quarry-hardrock a skos:Concept ;
    skos:broader gsqst:quarry ;
    skos:definition "A quarry in which the dominant commodities extracted over the life of the quarry are hardrock commodities. Classification is based on long term activity and annual variations may occur where a hardrock quarry does not predominantly produce hardrock in particular years."@en ;
    rdfs:isDefinedBy <http://linked.data.gov.au/def/geological-sites> ;
    skos:inScheme <http://linked.data.gov.au/def/geological-sites> ;
    skos:notation "qyhr" ;
    skos:prefLabel "Quarry - Hardrock"@en .

gsqst:quarry-sandgravel a skos:Concept ;
    skos:broader gsqst:quarry ;
    skos:definition "A quarry in which the dominant commodities extracted over the life of the quarry are sand and gravel commodities. Classification is based on long term activity and annual variations may occur where a sand and gravel quarry does not predominantly produce sand and gravel in particular years."@en ;
    rdfs:isDefinedBy <http://linked.data.gov.au/def/geological-sites> ;
    skos:inScheme <http://linked.data.gov.au/def/geological-sites> ;
    skos:notation "qysg" ;
    skos:prefLabel "Quarry - Sand and Gravel"@en .

gsqst:quarry-sand a skos:Concept ;
    skos:broader gsqst:quarry ;
    skos:definition "A quarry in which the dominant commodities extracted over the life of the quarry are sand commodities. Classification is based on long term activity and annual variations may occur where a sand quarry does not predominantly produce sand in particular years."@en ;
    rdfs:isDefinedBy <http://linked.data.gov.au/def/geological-sites> ;
    skos:inScheme <http://linked.data.gov.au/def/geological-sites> ;
    skos:notation "qysd" ;
    skos:prefLabel "Quarry - Sand"@en .

gsqst:quarry-gravel a skos:Concept ;
    skos:broader gsqst:quarry ;
    skos:definition "A quarry in which the dominant commodities extracted over the life of the quarry are gravel commodities. Classification is based on long term activity and annual variations may occur where a gravel quarry does not predominantly produce gravel in particular years."@en ;
    rdfs:isDefinedBy <http://linked.data.gov.au/def/geological-sites> ;
    skos:inScheme <http://linked.data.gov.au/def/geological-sites> ;
    skos:notation "qygv" ;
    skos:prefLabel "Quarry - Gravel"@en .

gsqst:pit a skos:Concept ;
    skos:altLabel "Gravel Scrape"@en,
        "Pits"@en ;
    skos:definition "A type of excavation or depression in the ground used for analysis or sample collection."@en ;
    rdfs:isDefinedBy <http://linked.data.gov.au/def/geological-sites> ;
    skos:inScheme <http://linked.data.gov.au/def/geological-sites> ;
    skos:notation "pt" ;
    skos:prefLabel "Pit"@en ;
    skos:topConceptOf <http://linked.data.gov.au/def/geological-sites> .

gsqst:geofeature a skos:Concept ;
    skos:definition "A site that is coincident with a geological feature, i.e. the spatial overlay that represents a geological feature in its entirety."@en ;
    rdfs:isDefinedBy <http://linked.data.gov.au/def/geological-sites> ;
    skos:inScheme <http://linked.data.gov.au/def/geological-sites> ;
    skos:notation "gf" ;
    skos:prefLabel "Geological Feature"@en ;
    skos:topConceptOf <http://linked.data.gov.au/def/geological-sites> .

gsqst:project-site a skos:Concept ;
    skos:altLabel "Project"@en,
        "Project Site"@en ;
    skos:definition "The location of a survey."@en ;
    rdfs:isDefinedBy <http://linked.data.gov.au/def/geological-sites> ;
    skos:inScheme <http://linked.data.gov.au/def/geological-sites> ;
    skos:notation "pj" ;
    skos:prefLabel "Survey Site"@en ;
    skos:topConceptOf <http://linked.data.gov.au/def/geological-sites> .

gsqst:trench a skos:Concept ;
    skos:altLabel "Box Cut"@en,
        "Costean"@en ;
    skos:definition "A narrow excavation in the ground."@en ;
    rdfs:isDefinedBy <http://linked.data.gov.au/def/geological-sites> ;
    skos:inScheme <http://linked.data.gov.au/def/geological-sites> ;
    skos:notation "th" ;
    skos:prefLabel "Trench"@en ;
    skos:topConceptOf <http://linked.data.gov.au/def/geological-sites> .

gsqst:administrative-area a skos:Concept ;
    skos:definition "An area of geological significance or definition, such as the location of a set of observations, surveys, or studies that is defined by an administrative or artificial boundary rather than a geological boundary."@en ;
    rdfs:isDefinedBy <http://linked.data.gov.au/def/geological-sites> ;
    skos:inScheme <http://linked.data.gov.au/def/geological-sites> ;
    skos:notation "aa" ;
    skos:prefLabel "Administrative Area"@en ;
    skos:topConceptOf <http://linked.data.gov.au/def/geological-sites> .

gsqst:map-sheet a skos:Concept ;
    skos:altLabel "Mapsheet"@en,
        "Map Series"@en ;
    skos:definition "A map series is a group of topographic or thematic maps or charts usually having the same scale and cartographic specifications, and with each sheet appropriately identified by its publisher as belonging to the same series. Map series occur when an area is to be covered by a map that, due to its scale, must be spread over several sheets. Nevertheless, the individual sheets of a map series can also be used quite independently, as they generally have full map surround details and legends. If a publisher produces several map series at different scales, then these series are called scale series."@en ;
    rdfs:isDefinedBy <http://linked.data.gov.au/def/geological-sites> ;
    skos:inScheme <http://linked.data.gov.au/def/geological-sites> ;
    skos:notation "ms" ;
    skos:prefLabel "Map Sheet"@en ;
    skos:broader gsqst:administrative-area .

gsqst:resource-authority a skos:Concept ;
    skos:altLabel "Permit"@en,
        "Tenure"@en ;
    skos:definition "Resource authorities are a license granted over a spatial region within the State of Queensland. Resource authorities govern the activities which can be conducted upon them. Activities include exploration, development, and extraction of a specific commodity or commodities."@en ;
    rdfs:isDefinedBy <http://linked.data.gov.au/def/geological-sites> ;
    skos:inScheme <http://linked.data.gov.au/def/geological-sites> ;
    skos:notation "ra" ;
    skos:prefLabel "Resource authority"@en ;
    skos:broader gsqst:administrative-area .

gsqst:lga a skos:Concept ;
    skos:definition "Local government area (LGA) is one of the spatial units defined under the non–ABS structures of the Australian Statistical Geography Standard (ASGS). Each area is governed by a local city, regional, town, or shire council."@en ;
    skos:altLabel "L.G.A."@en,
        "LGA"@en ;
    rdfs:isDefinedBy <http://linked.data.gov.au/def/geological-sites> ;
    skos:inScheme <http://linked.data.gov.au/def/geological-sites> ;
    skos:notation "lga" ;
    skos:prefLabel "Local Government Area"@en ;
    skos:broader gsqst:administrative-area .

#gsqst:wellbore a skos:Concept ;
#    skos:altLabel "Branch"@en,
#        "Sidetrack"@en ;
#    skos:definition "A Wellbore is a path of drilled footage, from the Borehole Origin (top/start) to a terminating point (bottom/end). There are one or more Wellbores in a planned or drilled Borehole, namely the original Wellbore, and a Wellbore for each intended, actual or accidental sidetrack. Each Wellbore has a unique terminating point. A deepening of an existing Wellbore is considered a new Wellbore with the same Borehole Origin. Source: PPDM What Is A  Well."@en ;
#    rdfs:isDefinedBy <http://linked.data.gov.au/def/geological-sites> ;
#    skos:inScheme <http://linked.data.gov.au/def/geological-sites> ;
#    skos:notation "wb" ;
#    skos:prefLabel "Wellbore"@en ;
#    skos:topConceptOf <http://linked.data.gov.au/def/geological-sites> .

gsqst:unknown a skos:Concept ;
    skos:altLabel "Null"@en ;
    skos:definition "The site of a sampling, survey, or observation in which the type of stie is unknown."@en ;
    rdfs:isDefinedBy <http://linked.data.gov.au/def/geological-sites> ;
    skos:inScheme <http://linked.data.gov.au/def/geological-sites> ;
    skos:notation "uk" ;
    skos:prefLabel "Unknown"@en ;
    skos:topConceptOf <http://linked.data.gov.au/def/geological-sites> .
