@prefix dc: <http://purl.org/dc/elements/1.1/> .
@prefix dcterms: <http://purl.org/dc/terms/> .
@prefix owl: <http://www.w3.org/2002/07/owl#> .
@prefix sdo: <http://schema.org/> .
@prefix skos: <http://www.w3.org/2004/02/skos/core#> .
@prefix rptdt: <http://linked.data.gov.au/def/report-detail-type/> .
@prefix rdfs: <http://www.w3.org/2000/01/rdf-schema#> .
@prefix xsd: <http://www.w3.org/2001/XMLSchema#> .

<http://linked.data.gov.au/def/report-detail-type> a owl:Ontology,
        skos:ConceptScheme ;
    dcterms:created "2020-04-29"^^xsd:date ;
    dcterms:creator <http://linked.data.gov.au/org/gsq> ;
    dcterms:modified "2020-07-07"^^xsd:date ;
    dcterms:publisher <http://linked.data.gov.au/org/gsq> ;
    dcterms:provenance "Compiled by the Geological Survey of Queensland" ;
    skos:definition "Miscellaneous details relating to reports and documents."@en ;
    skos:prefLabel "Report Detail Type"@en ;
    skos:hasTopConcept rptdt:activities,
            rptdt:address,
            rptdt:comments,
            rptdt:contact,
            rptdt:contracting-company,
            rptdt:email,
            rptdt:operating-company,
            rptdt:phone,
            rptdt:state,
            rptdt:suburb,
            rptdt:postcode,
            rptdt:project-name,
            rptdt:reportable-incident .

<http://linked.data.gov.au/org/gsq> a sdo:Organization ;
    sdo:name "Geological Survey of Queensland" ;
    sdo:url "http://www.business.qld.gov.au/industries/mining-energy-water/resources/geoscience-information/gsq"^^xsd:anyURI .
 
rptdt:activities a skos:Concept ;
    skos:altLabel "Plan"@en,
        "Planned Activities"@en,
        "Activities Undertaken"@en,
        "Activities to be Undertaken"@en ;
    skos:definition "A description of the activities referred to in the report or form. This may be a summary of activities undertaken, or a summary of planned activities."@en ;
    rdfs:isDefinedBy <http://linked.data.gov.au/def/report-detail-type> ;
    skos:inScheme <http://linked.data.gov.au/def/report-detail-type> ;
    skos:prefLabel "Activities"@en ;
    skos:topConceptOf <http://linked.data.gov.au/def/report-detail-type> .
  
rptdt:address a skos:Concept ;
    skos:definition "The address of the company submitting the report or form."@en ;
    rdfs:isDefinedBy <http://linked.data.gov.au/def/report-detail-type> ;
    skos:inScheme <http://linked.data.gov.au/def/report-detail-type> ;
    skos:prefLabel "Address"@en ;
    skos:topConceptOf <http://linked.data.gov.au/def/report-detail-type> .

rptdt:comments a skos:Concept ;
    skos:altLabel "Description"@en,
        "Remarks"@en,
        "Summary"@en ;         ;
    skos:definition "Any general commentary regarding the report or form, not otherwise captured."@en ;
    rdfs:isDefinedBy <http://linked.data.gov.au/def/report-detail-type> ;
    skos:inScheme <http://linked.data.gov.au/def/report-detail-type> ;
    skos:prefLabel "Comments"@en ;
    skos:topConceptOf <http://linked.data.gov.au/def/report-detail-type> .

rptdt:contact a skos:Concept ;
    skos:definition "The name of the individual contact for the report or form."@en ;
    rdfs:isDefinedBy <http://linked.data.gov.au/def/report-detail-type> ;
    skos:inScheme <http://linked.data.gov.au/def/report-detail-type> ;
    skos:prefLabel "Contact Name"@en ;
    skos:topConceptOf <http://linked.data.gov.au/def/report-detail-type> .
    
rptdt:contracting-company a skos:Concept ;
    skos:definition "The name of the company who conducted the activities referred to in the report or form."@en ;
    rdfs:isDefinedBy <http://linked.data.gov.au/def/report-detail-type> ;
    skos:inScheme <http://linked.data.gov.au/def/report-detail-type> ;
    skos:prefLabel "Contractor Name"@en ;
    skos:topConceptOf <http://linked.data.gov.au/def/report-detail-type> .

rptdt:email a skos:Concept ;
    skos:definition "The contact email address for the submitter of the report or form."@en ;
    rdfs:isDefinedBy <http://linked.data.gov.au/def/report-detail-type> ;
    skos:inScheme <http://linked.data.gov.au/def/report-detail-type> ;
    skos:prefLabel "E-mail"@en ;
    skos:topConceptOf <http://linked.data.gov.au/def/report-detail-type> .

rptdt:operating-company a skos:Concept ;
    skos:definition "The name of the company submitting the report or form."@en ;
    rdfs:isDefinedBy <http://linked.data.gov.au/def/report-detail-type> ;
    skos:inScheme <http://linked.data.gov.au/def/report-detail-type> ;
    skos:prefLabel "Company Name"@en ;
    skos:topConceptOf <http://linked.data.gov.au/def/report-detail-type> .

rptdt:suburb a skos:Concept ;
    skos:definition "The contact suburb for the submitter of the report or form."@en ;
    rdfs:isDefinedBy <http://linked.data.gov.au/def/report-detail-type> ;
    skos:inScheme <http://linked.data.gov.au/def/report-detail-type> ;
    skos:prefLabel "Suburb"@en ;
    skos:topConceptOf <http://linked.data.gov.au/def/report-detail-type> .

rptdt:postcode a skos:Concept ;
    skos:definition "The contact postcode for the submitter of the report or form."@en ;
    rdfs:isDefinedBy <http://linked.data.gov.au/def/report-detail-type> ;
    skos:inScheme <http://linked.data.gov.au/def/report-detail-type> ;
    skos:prefLabel "Postcode"@en ;
    skos:topConceptOf <http://linked.data.gov.au/def/report-detail-type> .

rptdt:state a skos:Concept ;
    skos:definition "The contact State for the submitter of the report or form."@en ;
    rdfs:isDefinedBy <http://linked.data.gov.au/def/report-detail-type> ;
    skos:inScheme <http://linked.data.gov.au/def/report-detail-type> ;
    skos:prefLabel "State"@en ;
    skos:topConceptOf <http://linked.data.gov.au/def/report-detail-type> .

rptdt:phone a skos:Concept ;
    skos:definition "The contact phone number for the submitter of the report or form."@en ;
    rdfs:isDefinedBy <http://linked.data.gov.au/def/report-detail-type> ;
    skos:inScheme <http://linked.data.gov.au/def/report-detail-type> ;
    skos:prefLabel "Phone Number"@en ;
    skos:topConceptOf <http://linked.data.gov.au/def/report-detail-type> .

rptdt:project-name a skos:Concept ;
    skos:definition "The name of the project to which a report relates."@en ;
    rdfs:isDefinedBy <http://linked.data.gov.au/def/report-detail-type> ;
    skos:inScheme <http://linked.data.gov.au/def/report-detail-type> ;
    skos:prefLabel "Project Name"@en ;
    skos:topConceptOf <http://linked.data.gov.au/def/report-detail-type> .

rptdt:reportable-incident a skos:Concept ;
    skos:definition "An indication of the occurrence of a reportable incident to be recorded in the report or form."@en ;
    rdfs:isDefinedBy <http://linked.data.gov.au/def/report-detail-type> ;
    skos:inScheme <http://linked.data.gov.au/def/report-detail-type> ;
    skos:prefLabel "Reportable Incident"@en ;
    skos:topConceptOf <http://linked.data.gov.au/def/report-detail-type> .
