@prefix svytp: <http://linked.data.gov.au/def/survey-type/> .
@prefix dc: <http://purl.org/dc/elements/1.1/> .
@prefix dcterms: <http://purl.org/dc/terms/> .
@prefix owl: <http://www.w3.org/2002/07/owl#> .
@prefix sdo: <http://schema.org/> .
@prefix skos: <http://www.w3.org/2004/02/skos/core#> .
@prefix rdfs: <http://www.w3.org/2000/01/rdf-schema#> .
@prefix xsd: <http://www.w3.org/2001/XMLSchema#> .

<http://linked.data.gov.au/def/survey-type> a owl:Ontology,
        skos:ConceptScheme ;
    dcterms:created "2020-02-05"^^xsd:date ;
    dcterms:creator <http://linked.data.gov.au/org/gsq> ;
    dcterms:modified "2020-05-14"^^xsd:date ;
    dcterms:publisher <http://linked.data.gov.au/org/gsq> ;
    dcterms:provenance "Compiled by the Geological Survey of Queensland" ;
    skos:definition "The one-off event examining a geological or administrative feature. The type of survey or sampling performed to investigate a feature, site, or sample. Surveys are activities that produce samples or make one-or-many observations."@en ;
    skos:hasTopConcept svytp:atmospheric,
        svytp:geochemistry,
        svytp:geophysical,
        svytp:geotechnical,
        svytp:hydrochemistry,
        svytp:petrophysical,
        svytp:physical-geology,
        svytp:seismic,
        svytp:spectral, 
        svytp:spatial,
        svytp:resource-production,
        svytp:resource-sales,
        svytp:resource-extractives ;
    skos:prefLabel "Survey Type"@en .

<http://linked.data.gov.au/org/gsq> a sdo:Organization ;
    sdo:name "Geological Survey of Queensland" ;
    sdo:url "http://www.business.qld.gov.au/industries/mining-energy-water/resources/geoscience-information/gsq"^^xsd:anyURI .

svytp:atmospheric a skos:Concept ;
    skos:definition "A survey measuring chemical and physical properties of the atmosphere."@en ;
    rdfs:isDefinedBy <http://linked.data.gov.au/def/survey-type> ;
    skos:inScheme <http://linked.data.gov.au/def/survey-type> ;
    skos:notation "at" ;
    skos:prefLabel "Atmospheric"@en ;
    skos:topConceptOf <http://linked.data.gov.au/def/survey-type> .

svytp:geochemistry a skos:Concept ;
    skos:definition "A survey where the chemical properties of rocks, soil, or other geological material is assessed to determine mineralogical and/or elemental composition."@en ;
    rdfs:isDefinedBy <http://linked.data.gov.au/def/survey-type> ;
    skos:inScheme <http://linked.data.gov.au/def/survey-type> ;
    skos:notation "gc" ;
    skos:prefLabel "Geochemistry"@en ;
    skos:topConceptOf <http://linked.data.gov.au/def/survey-type> .

svytp:geophysical a skos:Concept ;
    skos:definition "A survey where the geophysical properties of the earth is assessed."@en ;
    rdfs:isDefinedBy <http://linked.data.gov.au/def/survey-type> ;
    skos:inScheme <http://linked.data.gov.au/def/survey-type> ;
    skos:notation "gp" ;
    skos:prefLabel "Geophysical"@en ;
    skos:topConceptOf <http://linked.data.gov.au/def/survey-type> .
     
svytp:geotechnical a skos:Concept ;
    skos:altLabel "Geomechanical"@en ;
    skos:definition "A survey measuring the physical and mechanical properties of rocks, soil and earth material with particular focus on rock strength and competence."@en ;
    rdfs:isDefinedBy <http://linked.data.gov.au/def/survey-type> ;
    skos:inScheme <http://linked.data.gov.au/def/survey-type> ;
    skos:notation "gt" ;
    skos:prefLabel "Geotechnical"@en ;
    skos:topConceptOf <http://linked.data.gov.au/def/survey-type> .

svytp:hydrochemistry a skos:Concept ;
    skos:definition "A survey of the chemical and physical properties of surface or ground water."@en ;
    rdfs:isDefinedBy <http://linked.data.gov.au/def/survey-type> ;
    skos:inScheme <http://linked.data.gov.au/def/survey-type> ;
    skos:notation "hy" ;
    skos:prefLabel "Hydrochemistry"@en ;
    skos:topConceptOf <http://linked.data.gov.au/def/survey-type> .

svytp:petrophysical a skos:Concept ;
    skos:definition "A survey that records physical, chemical, electrical, or other properties of the rock/fluid mixtures. This may appliy to measurements derived via wireline logging, or properties analysed in a laboratory setting."@en ;
    rdfs:isDefinedBy <http://linked.data.gov.au/def/survey-type> ;
    skos:inScheme <http://linked.data.gov.au/def/survey-type> ;
    skos:notation "py" ;
    skos:prefLabel "Petrophysical"@en ;
    skos:topConceptOf <http://linked.data.gov.au/def/survey-type> .

svytp:physical-geology a skos:Concept ;
    skos:altLabel "Field Mapping"@en ;
    skos:definition "A survey of physical geological features such as outcrop samples, structural measurements, sedimentological and stratigraphic observations."@en ;
    rdfs:isDefinedBy <http://linked.data.gov.au/def/survey-type> ;
    skos:inScheme <http://linked.data.gov.au/def/survey-type> ;
    skos:notation "pg" ;
    skos:prefLabel "Physical Geology"@en ;
    skos:topConceptOf <http://linked.data.gov.au/def/survey-type> .

svytp:seismic a skos:Concept ;
    skos:definition "A survey using the interaction of seismic waves with sub-surface features of the earth to determine properties and morphology of those features."@en ;
    rdfs:isDefinedBy <http://linked.data.gov.au/def/survey-type> ;
    skos:inScheme <http://linked.data.gov.au/def/survey-type> ;
    skos:notation "ss" ;
    skos:prefLabel "Seismic"@en ;
    skos:topConceptOf <http://linked.data.gov.au/def/survey-type> .

svytp:spatial a skos:Concept ;
    skos:altLabel "Location Survey"@en ;
    skos:definition "A survey measuring the spatial characteristics of an object or region."@en ;
    rdfs:isDefinedBy <http://linked.data.gov.au/def/survey-type> ;
    skos:inScheme <http://linked.data.gov.au/def/survey-type> ;
    skos:notation "st" ;
    skos:prefLabel "Spatial"@en ;
    skos:topConceptOf <http://linked.data.gov.au/def/survey-type> .
    
svytp:spectral a skos:Concept ;
    skos:definition "A survey capturing image information and intensity-per-wavelength-band to be used for spectral analysis e.g. ASTER, MODIS."@en ;
    rdfs:isDefinedBy <http://linked.data.gov.au/def/survey-type> ;
    skos:inScheme <http://linked.data.gov.au/def/survey-type> ;
    skos:notation "sp" ;
    skos:prefLabel "Spectral"@en ;
    skos:topConceptOf <http://linked.data.gov.au/def/survey-type> .

svytp:resource-production a skos:Concept ;
    skos:definition "A survey capturing the production and processing statistics of a mine site in a given period."@en ;
    rdfs:isDefinedBy <http://linked.data.gov.au/def/survey-type> ;
    skos:inScheme <http://linked.data.gov.au/def/survey-type> ;
    skos:notation "rp" ;
    skos:prefLabel "Resource Production"@en ;
    skos:topConceptOf <http://linked.data.gov.au/def/survey-type> .

svytp:resource-sales a skos:Concept ;
    skos:definition "A survey capturing the sales statistics of a mine site in a given period."@en ;
    rdfs:isDefinedBy <http://linked.data.gov.au/def/survey-type> ;
    skos:inScheme <http://linked.data.gov.au/def/survey-type> ;
    skos:notation "rs" ;
    skos:prefLabel "Resource Sales"@en ;
    skos:topConceptOf <http://linked.data.gov.au/def/survey-type> .

svytp:resource-extractives a skos:Concept ;
    skos:definition "A survey capturing both production and sales statistics for a quarry in a given period."@en ;
    rdfs:isDefinedBy <http://linked.data.gov.au/def/survey-type> ;
    skos:inScheme <http://linked.data.gov.au/def/survey-type> ;
    skos:notation "re" ;
    skos:prefLabel "Resource Extractives"@en ;
    skos:topConceptOf <http://linked.data.gov.au/def/survey-type> .
