@prefix aac: <http://linked.data.gov.au/def/australian-phone-area-codes/> .
@prefix dcterms: <http://purl.org/dc/terms/> .
@prefix owl: <http://www.w3.org/2002/07/owl#> .
@prefix sdo: <http://schema.org/> .
@prefix skos: <http://www.w3.org/2004/02/skos/core#> .
@prefix rdfs: <http://www.w3.org/2000/01/rdf-schema#> .
@prefix xsd: <http://www.w3.org/2001/XMLSchema#> .

<http://linked.data.gov.au/def/australian-phone-area-codes> a owl:Ontology,
        skos:ConceptScheme ;
    dcterms:created "2020-03-25"^^xsd:date ;
    dcterms:creator <http://linked.data.gov.au/org/gsq> ;
    dcterms:modified "2020-03-25"^^xsd:date ;
    dcterms:publisher <http://linked.data.gov.au/org/gsq> ;
    dcterms:provenance "Derived from Australian Standard AS 4590.1:2017 citing The Australian Communications Media Authority (ACMA) Telecommunications Numbering Plan 2015." ;
    skos:definition "A two-digit-prefix code denoting the area in Australia to which a fixed telephone is registered."@en ;
    skos:prefLabel "Australian Telephone Area Codes"@en ;
    skos:hasTopConcept aac:02,
        aac:03,
        aac:07,
        aac:08 .

<http://linked.data.gov.au/org/gsq> a sdo:Organization ;
    sdo:name "Geological Survey of Queensland" ;
    sdo:url "http://www.business.qld.gov.au/industries/mining-energy-water/resources/geoscience-information/gsq"^^xsd:anyURI .

aac:02 a skos:Concept ;
    skos:altLabel "(02)"@en ;
    skos:definition "The Australian telephone area code for New South Wales and the Australian Captial Territory. (ACMA)"@en ;
    rdfs:isDefinedBy <http://linked.data.gov.au/def/australian-phone-area-codes> ;
    skos:inScheme <http://linked.data.gov.au/def/australian-phone-area-codes> ;
    skos:prefLabel "02"@en ;
    skos:topConceptOf <http://linked.data.gov.au/def/australian-phone-area-codes> .

aac:03 a skos:Concept ;
    skos:altLabel "(03)"@en ;
    skos:definition "The Australian telephone area code for Victoria and Tasmania. (ACMA)"@en ;
    rdfs:isDefinedBy <http://linked.data.gov.au/def/australian-phone-area-codes> ;
    skos:inScheme <http://linked.data.gov.au/def/australian-phone-area-codes> ;
    skos:prefLabel "03"@en ;
    skos:topConceptOf <http://linked.data.gov.au/def/australian-phone-area-codes> .

aac:07 a skos:Concept ;
    skos:altLabel "(07)"@en ;
    skos:definition "The Australian telephone area code for Queensland. (ACMA)"@en ;
    rdfs:isDefinedBy <http://linked.data.gov.au/def/australian-phone-area-codes> ;
    skos:inScheme <http://linked.data.gov.au/def/australian-phone-area-codes> ;
    skos:prefLabel "07"@en ;
    skos:topConceptOf <http://linked.data.gov.au/def/australian-phone-area-codes> .

aac:08 a skos:Concept ;
    skos:altLabel "(08)"@en ;
    skos:definition "The Australian telephone area code for South Australia and Western Australia, including Christmas Island  and Cocos (Keeling) Islands. (ACMA)"@en ;
    rdfs:isDefinedBy <http://linked.data.gov.au/def/australian-phone-area-codes> ;
    skos:inScheme <http://linked.data.gov.au/def/australian-phone-area-codes> ;
    skos:prefLabel "08"@en ;
    skos:topConceptOf <http://linked.data.gov.au/def/australian-phone-area-codes> .
