PREFIX dcterms: <http://purl.org/dc/terms/>
PREFIX gsqdt: <https://linked.data.gov.au/def/gsq-dataset-theme/>
PREFIX owl: <http://www.w3.org/2002/07/owl#>
PREFIX rdfs: <http://www.w3.org/2000/01/rdf-schema#>
PREFIX sdo: <https://schema.org/>
PREFIX skos: <http://www.w3.org/2004/02/skos/core#>
PREFIX xsd: <http://www.w3.org/2001/XMLSchema#>

gsqdt:activities-and-results
    a skos:Collection ;
    dcterms:provenance "Developed by the Geological Survey of Queensland." ;
    skos:definition "Primary results datasets that describe the geological features of interest and the activities that generate the results datasets."@en ;
    skos:member
        gsqdt:geoscience-data ,
        gsqdt:geoscience-project-data ,
        gsqdt:operational-data ,
        gsqdt:physical-samples ;
    skos:prefLabel "Activities and results"@en ;
.

gsqdt:ancillary-information
    a skos:Collection ;
    dcterms:provenance "Developed by the Geological Survey of Queensland." ;
    skos:definition "Data descriptive of the organisations involved in data collection and the administrative constraints and associations under which data is collected or related."@en ;
    skos:member
        gsqdt:administrative-data ,
        gsqdt:spatial-data ;
    skos:prefLabel "Ancillary information"@en ;
.

gsqdt:products-and-documents
    a skos:Collection ;
    dcterms:provenance "Developed by the Geological Survey of Queensland." ;
    skos:definition "The final products and official reports that synthesise the collected data into documentation that describe activities, results, contextual information, and any applicable interpretations."@en ;
    skos:member
        gsqdt:publications ,
        gsqdt:reports ;
    skos:prefLabel "Products and documents"@en ;
.

gsqdt:other
    a skos:Concept ;
    dcterms:provenance "Developed by the Geological Survey of Queensland." ;
    rdfs:isDefinedBy <https://linked.data.gov.au/def/gsq-dataset-theme> ;
    skos:definition "Any other metadata, data, or information that is not described by any of the other GSQ Dataset Themes."@en ;
    skos:inScheme <https://linked.data.gov.au/def/gsq-dataset-theme> ;
    skos:prefLabel "Other"@en ;
    skos:topConceptOf <https://linked.data.gov.au/def/gsq-dataset-theme> ;
.

gsqdt:resource-statistics
    a skos:Concept ;
    dcterms:provenance "Developed by the Geological Survey of Queensland." ;
    rdfs:isDefinedBy <https://linked.data.gov.au/def/gsq-dataset-theme> ;
    skos:definition "Statistical data and reports submitted to the department or generated by the department, particularly production, sales and reserve quantities."@en ;
    skos:inScheme <https://linked.data.gov.au/def/gsq-dataset-theme> ;
    skos:prefLabel "Resource statistics"@en ;
    skos:topConceptOf <https://linked.data.gov.au/def/gsq-dataset-theme> ;
.

gsqdt:administrative-data
    a skos:Concept ;
    dcterms:provenance "Developed by the Geological Survey of Queensland." ;
    rdfs:isDefinedBy <https://linked.data.gov.au/def/gsq-dataset-theme> ;
    skos:definition "Ancillary information regarding the administration of Queensland Resources such as administrative boundaries, resource permits, legislation, and information about organisations such as DNRME and GSQ."@en ;
    skos:inScheme <https://linked.data.gov.au/def/gsq-dataset-theme> ;
    skos:prefLabel "Administrative data"@en ;
    skos:topConceptOf <https://linked.data.gov.au/def/gsq-dataset-theme> ;
.

gsqdt:geoscience-data
    a skos:Concept ;
    dcterms:provenance "Developed by the Geological Survey of Queensland." ;
    rdfs:isDefinedBy <https://linked.data.gov.au/def/gsq-dataset-theme> ;
    skos:definition "Data and metadata that define and describe the geological attributes of a feature of interest."@en ;
    skos:inScheme <https://linked.data.gov.au/def/gsq-dataset-theme> ;
    skos:prefLabel "Geoscience data"@en ;
    skos:topConceptOf <https://linked.data.gov.au/def/gsq-dataset-theme> ;
.

gsqdt:geoscience-project-data
    a skos:Concept ;
    dcterms:provenance "Developed by the Geological Survey of Queensland." ;
    rdfs:isDefinedBy <https://linked.data.gov.au/def/gsq-dataset-theme> ;
    skos:definition "Data, metadata, and media describing project information such as the approval documentation, project planning, and activities performed to generate the primary geoscience data."@en ;
    skos:inScheme <https://linked.data.gov.au/def/gsq-dataset-theme> ;
    skos:prefLabel "Geoscience project data"@en ;
    skos:topConceptOf <https://linked.data.gov.au/def/gsq-dataset-theme> ;
.

gsqdt:operational-data
    a skos:Concept ;
    dcterms:provenance "Developed by the Geological Survey of Queensland." ;
    rdfs:isDefinedBy <https://linked.data.gov.au/def/gsq-dataset-theme> ;
    skos:definition "Data describing the operations of mining, drilling, processing, and sales operations e.g. borehole drilling, pipeline operations, processing facility operations."@en ;
    skos:inScheme <https://linked.data.gov.au/def/gsq-dataset-theme> ;
    skos:prefLabel "Operational data"@en ;
    skos:topConceptOf <https://linked.data.gov.au/def/gsq-dataset-theme> ;
.

gsqdt:physical-samples
    a skos:Concept ;
    dcterms:provenance "Developed by the Geological Survey of Queensland." ;
    rdfs:isDefinedBy <https://linked.data.gov.au/def/gsq-dataset-theme> ;
    skos:definition "Data and metadata pertaining to physical samples taken during geoscience data acquisition e.g. drill core, rock chips, rock samples from outcrop, soil, sediment, water, drilling fluids, hydrocarbons etc."@en ;
    skos:inScheme <https://linked.data.gov.au/def/gsq-dataset-theme> ;
    skos:prefLabel "Physical samples"@en ;
    skos:topConceptOf <https://linked.data.gov.au/def/gsq-dataset-theme> ;
.

gsqdt:publications
    a skos:Concept ;
    dcterms:provenance "Developed by the Geological Survey of Queensland." ;
    rdfs:isDefinedBy <https://linked.data.gov.au/def/gsq-dataset-theme> ;
    skos:definition "Publications that describe the geology, resource potential, or other areas of departmental interest such as books, journals, periodicals, presentations, posters, academic publications, or multimedia products."@en ;
    skos:inScheme <https://linked.data.gov.au/def/gsq-dataset-theme> ;
    skos:prefLabel "Publications"@en ;
    skos:topConceptOf <https://linked.data.gov.au/def/gsq-dataset-theme> ;
.

gsqdt:reports
    a skos:Concept ;
    dcterms:provenance "Developed by the Geological Survey of Queensland." ;
    rdfs:isDefinedBy <https://linked.data.gov.au/def/gsq-dataset-theme> ;
    skos:definition "Reports lodged as part of an approved study or activity, commonly for the purpose of compliance with permit grant and retention conditions. These reports may be permit based such as resource authority annual reports, activity based such as well completion reports, or non-tenure reports such as departmental survey reports or academic studies."@en ;
    skos:inScheme <https://linked.data.gov.au/def/gsq-dataset-theme> ;
    skos:prefLabel "Reports"@en ;
    skos:topConceptOf <https://linked.data.gov.au/def/gsq-dataset-theme> ;
.

gsqdt:spatial-data
    a skos:Concept ;
    dcterms:provenance "Developed by the Geological Survey of Queensland." ;
    rdfs:isDefinedBy <https://linked.data.gov.au/def/gsq-dataset-theme> ;
    skos:definition "Spatial data including maps, aerial and satellite imagery, and files for use in GIS software."@en ;
    skos:inScheme <https://linked.data.gov.au/def/gsq-dataset-theme> ;
    skos:prefLabel "Spatial data"@en ;
    skos:topConceptOf <https://linked.data.gov.au/def/gsq-dataset-theme> ;
.

<https://linked.data.gov.au/org/gsq>
    a sdo:Organization ;
    sdo:name "Geological Survey of Queensland" ;
    sdo:url "http://www.business.qld.gov.au/industries/mining-energy-water/resources/geoscience-information/gsq"^^xsd:anyURI ;
.

<https://linked.data.gov.au/def/gsq-dataset-theme>
    a
        owl:Ontology ,
        skos:ConceptScheme ;
    dcterms:created "2019-10-02T15:00:47"^^xsd:dateTime ;
    dcterms:creator <https://linked.data.gov.au/org/gsq> ;
    dcterms:modified "2023-03-16"^^xsd:date ;
    dcterms:provenance "Developed by the Geological Survey of Queensland." ;
    dcterms:publisher <https://linked.data.gov.au/org/gsq> ;
    skos:definition "A list of broad thematic descriptions of datasets created, received, and held by the Geological Survey of Queensland."@en ;
    skos:hasTopConcept
        gsqdt:administrative-data ,
        gsqdt:geoscience-data ,
        gsqdt:geoscience-project-data ,
        gsqdt:operational-data ,
        gsqdt:other ,
        gsqdt:physical-samples ,
        gsqdt:publications ,
        gsqdt:reports ,
        gsqdt:resource-statistics ,
        gsqdt:spatial-data ;
    skos:prefLabel "GSQ Dataset Themes"@en ;
.

