PREFIX dcterms: <http://purl.org/dc/terms/>
PREFIX orgnt: <https://linked.data.gov.au/def/organisation-name-types/>
PREFIX owl: <http://www.w3.org/2002/07/owl#>
PREFIX rdfs: <http://www.w3.org/2000/01/rdf-schema#>
PREFIX sdo: <https://schema.org/>
PREFIX skos: <http://www.w3.org/2004/02/skos/core#>
PREFIX xsd: <http://www.w3.org/2001/XMLSchema#>

orgnt:legal-organisation-name
    a skos:Concept ;
    dcterms:provenance "Derived from Australian Standard AS 4590.1:2017." ;
    rdfs:isDefinedBy <https://linked.data.gov.au/def/organisation-name-types> ;
    skos:definition "This is the name of the owner of the organisation that appears on all legal papers (AS4590.1:2017)."@en ;
    skos:inScheme <https://linked.data.gov.au/def/organisation-name-types> ;
    skos:notation "LGL" ;
    skos:prefLabel "Legal Organisation Name"@en ;
    skos:topConceptOf <https://linked.data.gov.au/def/organisation-name-types> ;
.

orgnt:main-organisation
    a skos:Concept ;
    dcterms:provenance "Derived from Australian Standard AS 4590.1:2017." ;
    rdfs:isDefinedBy <https://linked.data.gov.au/def/organisation-name-types> ;
    skos:definition "Main name of the organisation. This is the name of the entity that appears on all official documents or legal papers. May be the registered Business name where it is different to the Trading name (AS4590.1:2017)."@en ;
    skos:inScheme <https://linked.data.gov.au/def/organisation-name-types> ;
    skos:notation "MN" ;
    skos:prefLabel "Main Organisation"@en ;
    skos:topConceptOf <https://linked.data.gov.au/def/organisation-name-types> ;
.

orgnt:main-trading-name
    a skos:Concept ;
    dcterms:provenance "Derived from Australian Standard AS 4590.1:2017." ;
    rdfs:isDefinedBy <https://linked.data.gov.au/def/organisation-name-types> ;
    skos:altLabel "Trading Name"@en ;
    skos:definition "The main name that the organisation trades under or the name by which suppliers or customers know the organisation (AS4590.1:2017)."@en ;
    skos:inScheme <https://linked.data.gov.au/def/organisation-name-types> ;
    skos:notation "MTR" ;
    skos:prefLabel "Main Trading Name"@en ;
    skos:topConceptOf <https://linked.data.gov.au/def/organisation-name-types> ;
.

orgnt:management-accounting-unit
    a skos:Concept ;
    dcterms:provenance "Derived from Australian Standard AS 4590.1:2017." ;
    rdfs:isDefinedBy <https://linked.data.gov.au/def/organisation-name-types> ;
    skos:definition "Management accounting unit. These are principal business units for which regular accounts are maintained, e.g. a division of a large business such as BHP's Steel Division. MAUs are ABS defined but are a popular way for large businesses to manage diverse undertakings (AS4590.1:2017)."@en ;
    skos:inScheme <https://linked.data.gov.au/def/organisation-name-types> ;
    skos:notation "MAU" ;
    skos:prefLabel "Management Accounting Unit"@en ;
    skos:topConceptOf <https://linked.data.gov.au/def/organisation-name-types> ;
.

orgnt:other-name
    a skos:Concept ;
    dcterms:provenance "Derived from Australian Standard AS 4590.1:2017." ;
    rdfs:isDefinedBy <https://linked.data.gov.au/def/organisation-name-types> ;
    skos:definition "Other name type not listed, e.g. sales and marketing  (AS4590.1:2017)."@en ;
    skos:inScheme <https://linked.data.gov.au/def/organisation-name-types> ;
    skos:notation "OTH" ;
    skos:prefLabel "Other Name"@en ;
    skos:topConceptOf <https://linked.data.gov.au/def/organisation-name-types> ;
.

orgnt:other-trading-name
    a skos:Concept ;
    dcterms:provenance "Derived from Australian Standard AS 4590.1:2017." ;
    rdfs:isDefinedBy <https://linked.data.gov.au/def/organisation-name-types> ;
    skos:definition "Alternative trading name for an organisation that is not registered (AS4590.1:2017)."@en ;
    skos:inScheme <https://linked.data.gov.au/def/organisation-name-types> ;
    skos:notation "OTR" ;
    skos:prefLabel "Other Trading Name"@en ;
    skos:topConceptOf <https://linked.data.gov.au/def/organisation-name-types> ;
.

orgnt:unknown
    a skos:Concept ;
    dcterms:provenance "Derived from Australian Standard AS 4590.1:2017." ;
    rdfs:isDefinedBy <https://linked.data.gov.au/def/organisation-name-types> ;
    skos:definition "There is no information about the name type (AS4590.1:2017)."@en ;
    skos:inScheme <https://linked.data.gov.au/def/organisation-name-types> ;
    skos:notation "UNK" ;
    skos:prefLabel "Unknown"@en ;
    skos:topConceptOf <https://linked.data.gov.au/def/organisation-name-types> ;
.

<https://linked.data.gov.au/org/gsq>
    a sdo:Organization ;
    sdo:name "Geological Survey of Queensland" ;
    sdo:url "http://www.business.qld.gov.au/industries/mining-energy-water/resources/geoscience-information/gsq"^^xsd:anyURI ;
.

<https://linked.data.gov.au/def/organisation-name-types>
    a
        owl:Ontology ,
        skos:ConceptScheme ;
    dcterms:created "2020-03-25"^^xsd:date ;
    dcterms:creator <https://linked.data.gov.au/org/gsq> ;
    dcterms:modified "2023-03-16"^^xsd:date ;
    dcterms:provenance "Derived from Australian Standard AS 4590.1:2017." ;
    dcterms:publisher <https://linked.data.gov.au/org/gsq> ;
    skos:definition "Types of names provided by organisations."@en ;
    skos:hasTopConcept
        orgnt:legal-organisation-name ,
        orgnt:main-organisation ,
        orgnt:main-trading-name ,
        orgnt:management-accounting-unit ,
        orgnt:other-name ,
        orgnt:other-trading-name ,
        orgnt:unknown ;
    skos:prefLabel "Organisation Name Types"@en ;
.

