PREFIX dcterms: <http://purl.org/dc/terms/>
PREFIX expt: <http://linked.data.gov.au/def/qld-export-terminals/>
PREFIX owl: <http://www.w3.org/2002/07/owl#>
PREFIX rdfs: <http://www.w3.org/2000/01/rdf-schema#>
PREFIX sdo: <http://schema.org/>
PREFIX skos: <http://www.w3.org/2004/02/skos/core#>
PREFIX xsd: <http://www.w3.org/2001/XMLSchema#>

expt:coal-terminals
    a skos:Collection ;
    dcterms:provenance "Compiled by the Geological Survey of Queensland" ;
    skos:definition "The ports, terminals, and land based transport methods applicable to the shipment of coal in Queensland."@en ;
    skos:member
        expt:abbot-point ,
        expt:belt ,
        expt:dalrymple-bay ,
        expt:gladstone-port ,
        expt:hay-point ,
        expt:port-of-brisbane ,
        expt:rail ,
        expt:road ;
    skos:prefLabel "Queensland Coal Ports and Terminals"@en ;
.

expt:abbot-point
    a skos:Concept ;
    dcterms:provenance "Compiled by the Geological Survey of Queensland" ;
    rdfs:isDefinedBy <http://linked.data.gov.au/def/qld-export-terminals> ;
    skos:definition "The Abbot Point Port situated approximately 25 kilometres (16 mi) north-west of the township of Bowen (Queensland) including the North Queensland Export Terminal."@en ;
    skos:inScheme <http://linked.data.gov.au/def/qld-export-terminals> ;
    skos:prefLabel "Abbot Point"@en ;
.

expt:belt
    a skos:Concept ;
    dcterms:provenance "Compiled by the Geological Survey of Queensland" ;
    rdfs:isDefinedBy <http://linked.data.gov.au/def/qld-export-terminals> ;
    skos:altLabel "BELT"@en ;
    skos:definition "Domestic land-based transport that primarily uses short-distance conveyor belts."@en ;
    skos:inScheme <http://linked.data.gov.au/def/qld-export-terminals> ;
    skos:prefLabel "Belt"@en ;
.

expt:dalrymple-bay
    a skos:Concept ;
    dcterms:provenance "Compiled by the Geological Survey of Queensland" ;
    rdfs:isDefinedBy <http://linked.data.gov.au/def/qld-export-terminals> ;
    skos:definition "The Dalrymple Bay Coal Terminal situated in the Mackay Region (Queensland)."@en ;
    skos:inScheme <http://linked.data.gov.au/def/qld-export-terminals> ;
    skos:prefLabel "Dalrymple Bay"@en ;
.

expt:gladstone-port
    a skos:Concept ;
    dcterms:provenance "Compiled by the Geological Survey of Queensland" ;
    rdfs:isDefinedBy <http://linked.data.gov.au/def/qld-export-terminals> ;
    skos:altLabel "Port of Gladstone"@en ;
    skos:definition "The Port of Gladstone multi-commodity port located in the Gladstone Region (Queensland)."@en ;
    skos:inScheme <http://linked.data.gov.au/def/qld-export-terminals> ;
    skos:prefLabel "Gladstone Port"@en ;
.

expt:hay-point
    a skos:Concept ;
    dcterms:provenance "Compiled by the Geological Survey of Queensland" ;
    rdfs:isDefinedBy <http://linked.data.gov.au/def/qld-export-terminals> ;
    skos:definition "The Hay Point Services Coal Terminal situated in the Mackay Region (Queensland)."@en ;
    skos:inScheme <http://linked.data.gov.au/def/qld-export-terminals> ;
    skos:prefLabel "Hay Point"@en ;
.

expt:port-of-brisbane
    a skos:Concept ;
    dcterms:provenance "Compiled by the Geological Survey of Queensland" ;
    rdfs:isDefinedBy <http://linked.data.gov.au/def/qld-export-terminals> ;
    skos:definition "The Port of Brisbane located on the east coast of Australia, within the City of Brisbane and at the mouth of the Brisbane River, adjacent to Moreton Bay."@en ;
    skos:inScheme <http://linked.data.gov.au/def/qld-export-terminals> ;
    skos:prefLabel "Port of Brisbane"@en ;
.

expt:rail
    a skos:Concept ;
    dcterms:provenance "Compiled by the Geological Survey of Queensland" ;
    rdfs:isDefinedBy <http://linked.data.gov.au/def/qld-export-terminals> ;
    skos:altLabel "RAIL"@en ;
    skos:definition "Domestic land-based transport that primarily uses the Queensland rail network."@en ;
    skos:inScheme <http://linked.data.gov.au/def/qld-export-terminals> ;
    skos:prefLabel "Rail"@en ;
.

expt:road
    a skos:Concept ;
    dcterms:provenance "Compiled by the Geological Survey of Queensland" ;
    rdfs:isDefinedBy <http://linked.data.gov.au/def/qld-export-terminals> ;
    skos:altLabel "ROAD"@en ;
    skos:definition "Domestic land-based transport that primarily uses the Queensland road network."@en ;
    skos:inScheme <http://linked.data.gov.au/def/qld-export-terminals> ;
    skos:prefLabel "Road"@en ;
.

<https://linked.data.gov.au/org/gsq>
    a sdo:Organization ;
    sdo:name "Geological Survey of Queensland" ;
    sdo:url "http://www.business.qld.gov.au/industries/mining-energy-water/resources/geoscience-information/gsq"^^xsd:anyURI ;
.

<http://linked.data.gov.au/def/qld-export-terminals>
    a
        owl:Ontology ,
        skos:ConceptScheme ;
    dcterms:created "2020-04-07"^^xsd:date ;
    dcterms:creator <https://linked.data.gov.au/org/gsq> ;
    dcterms:modified "2023-03-16"^^xsd:date ;
    dcterms:provenance "Compiled by the Geological Survey of Queensland" ;
    dcterms:publisher <https://linked.data.gov.au/org/gsq> ;
    skos:definition "Export terminals for the shipment of resources originating in the state of queensland and the types of land based transport."@en ;
    skos:hasTopConcept
        expt:abbot-point ,
        expt:belt ,
        expt:dalrymple-bay ,
        expt:gladstone-port ,
        expt:hay-point ,
        expt:port-of-brisbane ,
        expt:rail ,
        expt:road ;
    skos:prefLabel "Queensland Export Ports and Terminals"@en ;
.

