@prefix dc: <http://purl.org/dc/elements/1.1/> .
@prefix dcterms: <http://purl.org/dc/terms/> .
@prefix owl: <http://www.w3.org/2002/07/owl#> .
@prefix qldutm: <http://linked.data.gov.au/def/qld-utm-zones/> .
@prefix sdo: <http://schema.org/> .
@prefix skos: <http://www.w3.org/2004/02/skos/core#> .
@prefix rdfs: <http://www.w3.org/2000/01/rdf-schema#> .
@prefix xsd: <http://www.w3.org/2001/XMLSchema#> .

<http://linked.data.gov.au/def/qld-utm-zones> a owl:Ontology , skos:ConceptScheme ;
    dcterms:created "2020-01-31T08:40:52"^^xsd:dateTime ;
    dcterms:creator <http://linked.data.gov.au/org/gsq> ;
    dcterms:publisher <http://linked.data.gov.au/org/gsq> ;
    dcterms:modified "2020-01-31T08:40:52"^^xsd:dateTime ;
    dcterms:provenance "Concepts extracted from OGC sources" ;
    skos:definition "The universal transverse mercator (UTM) zones used and referred to within Queensland. The UTM system divides the Earth into 60 zones, each 6 degrees of longitude in width. Zone 1 covers longitude 180 to 174 W; zone numbering increases eastward to zone 60, which covers longitude 174 to 180E. The polar regions south of 80S and north of 84N are excluded."@en ;
    skos:hasTopConcept qldutm:z54,
        qldutm:z55,
        qldutm:z56 ;
    skos:prefLabel "QLD UTM Zones"@en .

<http://linked.data.gov.au/org/gsq> a sdo:Organization ;
    sdo:name "Geological Survey of Queensland" ;
    sdo:url "http://www.business.qld.gov.au/industries/mining-energy-water/resources/geoscience-information/gsq"^^xsd:anyURI .

qldutm:z54 a skos:Concept ;
    skos:definition "The 54th UTM zone spanning from 138 to 144 degrees of longitude east. Central Meridian 141 degrees east"@en ;
    rdfs:isDefinedBy <http://linked.data.gov.au/def/qld-utm-zones> ;
    skos:inScheme <http://linked.data.gov.au/def/qld-utm-zones> ;
    skos:prefLabel "Z54"@en ;
    skos:topConceptOf <http://linked.data.gov.au/def/qld-utm-zones> .

qldutm:z55 a skos:Concept ;
    skos:definition "The 55th UTM zone spanning from 144 to 150 degrees of longitude east. Central Meridian 147 degrees east"@en ;
    rdfs:isDefinedBy <http://linked.data.gov.au/def/qld-utm-zones> ;
    skos:inScheme <http://linked.data.gov.au/def/qld-utm-zones> ;
    skos:prefLabel "Z55"@en ;
    skos:topConceptOf <http://linked.data.gov.au/def/qld-utm-zones> .

qldutm:z56 a skos:Concept ;
    skos:definition "The 56th UTM zone spanning from 150 to 156 degrees of longitude east. Central Meridian 153 degrees east"@en ;
    rdfs:isDefinedBy <http://linked.data.gov.au/def/qld-utm-zones> ;
    skos:inScheme <http://linked.data.gov.au/def/qld-utm-zones> ;
    skos:prefLabel "Z56"@en ;
    skos:topConceptOf <http://linked.data.gov.au/def/qld-utm-zones> .

