PREFIX dcterms: <http://purl.org/dc/terms/>
PREFIX owl: <http://www.w3.org/2002/07/owl#>
PREFIX rdfs: <http://www.w3.org/2000/01/rdf-schema#>
PREFIX rptst: <http://linked.data.gov.au/def/report-status/>
PREFIX sdo: <http://schema.org/>
PREFIX skos: <http://www.w3.org/2004/02/skos/core#>
PREFIX xsd: <http://www.w3.org/2001/XMLSchema#>

rptst:abandoned
    a skos:Concept ;
    dcterms:provenance "Compiled by the Geological Survey of Queensland" ;
    rdfs:isDefinedBy <http://linked.data.gov.au/def/report-status> ;
    skos:altLabel "Cancelled"@en ;
    skos:definition "The report was saved in the lodgement portal but not submitted within 90 days. Any S3 resources have been subsequently deleted."@en ;
    skos:inScheme <http://linked.data.gov.au/def/report-status> ;
    skos:prefLabel "Abandoned"@en ;
    skos:topConceptOf <http://linked.data.gov.au/def/report-status> ;
.

rptst:in-progress
    a skos:Concept ;
    dcterms:provenance "Compiled by the Geological Survey of Queensland" ;
    rdfs:isDefinedBy <http://linked.data.gov.au/def/report-status> ;
    skos:altLabel
        "Pending"@en ,
        "Saved"@en ,
        "Started"@en ;
    skos:definition "The report is in-progress and saved in the lodgement portal awaiting submission."@en ;
    skos:inScheme <http://linked.data.gov.au/def/report-status> ;
    skos:prefLabel "In-Progress"@en ;
    skos:topConceptOf <http://linked.data.gov.au/def/report-status> ;
.

rptst:screening
    a skos:Concept ;
    dcterms:provenance "Compiled by the Geological Survey of Queensland" ;
    rdfs:isDefinedBy <http://linked.data.gov.au/def/report-status> ;
    skos:definition "The report is held by the department for examination prior to submission being allowed"@en ;
    skos:inScheme <http://linked.data.gov.au/def/report-status> ;
    skos:prefLabel "Screening"@en ;
    skos:topConceptOf <http://linked.data.gov.au/def/report-status> ;
.

rptst:submitted
    a skos:Concept ;
    dcterms:provenance "Compiled by the Geological Survey of Queensland" ;
    rdfs:isDefinedBy <http://linked.data.gov.au/def/report-status> ;
    skos:definition "The report has been sucessfully submitted."@en ;
    skos:inScheme <http://linked.data.gov.au/def/report-status> ;
    skos:prefLabel "Submitted"@en ;
    skos:topConceptOf <http://linked.data.gov.au/def/report-status> ;
.

<https://linked.data.gov.au/org/gsq>
    a sdo:Organization ;
    sdo:name "Geological Survey of Queensland" ;
    sdo:url "http://www.business.qld.gov.au/industries/mining-energy-water/resources/geoscience-information/gsq"^^xsd:anyURI ;
.

<http://linked.data.gov.au/def/report-status>
    a
        owl:Ontology ,
        skos:ConceptScheme ;
    dcterms:created "2020-03-03T13:30:19"^^xsd:dateTime ;
    dcterms:creator <https://linked.data.gov.au/org/gsq> ;
    dcterms:modified "2020-03-03T13:30:19"^^xsd:dateTime ;
    dcterms:provenance "Compiled by the Geological Survey of Queensland" ;
    dcterms:publisher <https://linked.data.gov.au/org/gsq> ;
    skos:definition "The status of a report during the submission process in the GSQ Open Data Portal Lodegement System."@en ;
    skos:hasTopConcept
        rptst:in-progress ,
        rptst:screening ,
        rptst:submitted ;
    skos:prefLabel "Report Status"@en ;
.

