PREFIX dcterms: <http://purl.org/dc/terms/>
PREFIX owl: <http://www.w3.org/2002/07/owl#>
PREFIX rdfs: <http://www.w3.org/2000/01/rdf-schema#>
PREFIX sdo: <http://schema.org/>
PREFIX skos: <http://www.w3.org/2004/02/skos/core#>
PREFIX smprep: <https://linked.data.gov.au/def/sample-preparation-methods/>
PREFIX xsd: <http://www.w3.org/2001/XMLSchema#>

smprep:mine-processing
    a skos:Collection ;
    dcterms:provenance "Compiled by the Geological Survey of Queensland" ;
    skos:definition "Sample preparation steps and multi-step processes that concentrate, refine, or prepare a raw material into a saleable product."@en ;
    skos:member
        smprep:beneficiate ,
        smprep:concentrate ,
        smprep:crush-sort ,
        smprep:cut ,
        smprep:gravity-concentrate ,
        smprep:partial-cut ,
        smprep:refine ,
        smprep:refining-byproduct ,
        smprep:rough-extract ,
        smprep:smelt ,
        smprep:smelt-byproduct ,
        smprep:unprocessed ,
        smprep:unspecified ;
    skos:prefLabel "Mine Processing"@en ;
.

smprep:acidify
    a skos:Concept ;
    dcterms:provenance "Compiled by the Geological Survey of Queensland" ;
    rdfs:isDefinedBy <https://linked.data.gov.au/def/sample-preparation-methods> ;
    skos:altLabel "Sour"@en ;
    skos:definition "The process of making a material more acidic."@en ;
    skos:inScheme <https://linked.data.gov.au/def/sample-preparation-methods> ;
    skos:prefLabel "Acidify"@en ;
    skos:topConceptOf <https://linked.data.gov.au/def/sample-preparation-methods> ;
.

smprep:aggregate
    a skos:Concept ;
    dcterms:provenance "Compiled by the Geological Survey of Queensland" ;
    rdfs:isDefinedBy <https://linked.data.gov.au/def/sample-preparation-methods> ;
    skos:altLabel "Compile"@en ;
    skos:definition "To collect or gather into a mass or whole"@en ;
    skos:inScheme <https://linked.data.gov.au/def/sample-preparation-methods> ;
    skos:prefLabel "Aggregate"@en ;
    skos:topConceptOf <https://linked.data.gov.au/def/sample-preparation-methods> ;
.

smprep:chelate
    a skos:Concept ;
    dcterms:provenance "Compiled by the Geological Survey of Queensland" ;
    rdfs:isDefinedBy <https://linked.data.gov.au/def/sample-preparation-methods> ;
    skos:definition "A chemical process to cluster metallic ions."@en ;
    skos:inScheme <https://linked.data.gov.au/def/sample-preparation-methods> ;
    skos:prefLabel "Chelate"@en ;
    skos:topConceptOf <https://linked.data.gov.au/def/sample-preparation-methods> ;
.

smprep:compress
    a skos:Concept ;
    dcterms:provenance "Compiled by the Geological Survey of Queensland" ;
    rdfs:isDefinedBy <https://linked.data.gov.au/def/sample-preparation-methods> ;
    skos:altLabel
        "Compression"@en ,
        "Pressurisation"@en ;
    skos:definition "The action of increasing pressure on a sample."@en ;
    skos:inScheme <https://linked.data.gov.au/def/sample-preparation-methods> ;
    skos:prefLabel "Compress"@en ;
    skos:topConceptOf <https://linked.data.gov.au/def/sample-preparation-methods> ;
.

smprep:condense
    a skos:Concept ;
    dcterms:provenance "Compiled by the Geological Survey of Queensland" ;
    rdfs:isDefinedBy <https://linked.data.gov.au/def/sample-preparation-methods> ;
    skos:definition "To change a gas to a liquid. Typically through decreasing temperature or increasing pressure."@en ;
    skos:inScheme <https://linked.data.gov.au/def/sample-preparation-methods> ;
    skos:prefLabel "Condense"@en ;
    skos:topConceptOf <https://linked.data.gov.au/def/sample-preparation-methods> ;
.

smprep:cool
    a skos:Concept ;
    dcterms:provenance "Compiled by the Geological Survey of Queensland" ;
    rdfs:isDefinedBy <https://linked.data.gov.au/def/sample-preparation-methods> ;
    skos:definition "The process of reducing the sample temperature."@en ;
    skos:inScheme <https://linked.data.gov.au/def/sample-preparation-methods> ;
    skos:prefLabel "Cool"@en ;
    skos:topConceptOf <https://linked.data.gov.au/def/sample-preparation-methods> ;
.

smprep:cupellation
    a skos:Concept ;
    dcterms:provenance "Compiled by the Geological Survey of Queensland" ;
    rdfs:isDefinedBy <https://linked.data.gov.au/def/sample-preparation-methods> ;
    skos:broader smprep:melt ;
    skos:definition "The refining process in metallurgy where ores or alloyed metals are treated under very high temperatures and have controlled operations to separate noble metals, like gold and silver, from base metals, like lead, copper, zinc, arsenic, antimony, or bismuth, present in the ore."@en ;
    skos:inScheme <https://linked.data.gov.au/def/sample-preparation-methods> ;
    skos:prefLabel "Cupellation"@en ;
.

smprep:deacidify
    a skos:Concept ;
    dcterms:provenance "Compiled by the Geological Survey of Queensland" ;
    rdfs:isDefinedBy <https://linked.data.gov.au/def/sample-preparation-methods> ;
    skos:altLabel "Sweeten"@en ;
    skos:definition "The process of making a material more alkaline."@en ;
    skos:inScheme <https://linked.data.gov.au/def/sample-preparation-methods> ;
    skos:prefLabel "Deacidify"@en ;
    skos:topConceptOf <https://linked.data.gov.au/def/sample-preparation-methods> ;
.

smprep:decompress
    a skos:Concept ;
    dcterms:provenance "Compiled by the Geological Survey of Queensland" ;
    rdfs:isDefinedBy <https://linked.data.gov.au/def/sample-preparation-methods> ;
    skos:altLabel
        "Decompression"@en ,
        "Depressurisation"@en ;
    skos:definition "The action of decreasing pressure on a sample."@en ;
    skos:inScheme <https://linked.data.gov.au/def/sample-preparation-methods> ;
    skos:prefLabel "Decompress"@en ;
    skos:topConceptOf <https://linked.data.gov.au/def/sample-preparation-methods> ;
.

smprep:deposit
    a skos:Concept ;
    dcterms:provenance "Compiled by the Geological Survey of Queensland" ;
    rdfs:isDefinedBy <https://linked.data.gov.au/def/sample-preparation-methods> ;
    skos:definition "To change a gas to a solid. Typically through decreasing temperature or increasing pressure."@en ;
    skos:inScheme <https://linked.data.gov.au/def/sample-preparation-methods> ;
    skos:prefLabel "Deposit"@en ;
    skos:topConceptOf <https://linked.data.gov.au/def/sample-preparation-methods> ;
.

smprep:dessicate
    a skos:Concept ;
    dcterms:provenance "Compiled by the Geological Survey of Queensland" ;
    rdfs:isDefinedBy <https://linked.data.gov.au/def/sample-preparation-methods> ;
    skos:altLabel
        "Dehydrating"@en ,
        "Drying"@en ;
    skos:definition "The removal of a liquid component from a solid."@en ;
    skos:inScheme <https://linked.data.gov.au/def/sample-preparation-methods> ;
    skos:prefLabel "Dessicate"@en ;
    skos:topConceptOf <https://linked.data.gov.au/def/sample-preparation-methods> ;
.

smprep:dilute
    a skos:Concept ;
    dcterms:provenance "Compiled by the Geological Survey of Queensland" ;
    rdfs:isDefinedBy <https://linked.data.gov.au/def/sample-preparation-methods> ;
    skos:definition "Preparation by addition of the solvent or diluting agent(s)."@en ;
    skos:inScheme <https://linked.data.gov.au/def/sample-preparation-methods> ;
    skos:prefLabel "Dilute"@en ;
    skos:topConceptOf <https://linked.data.gov.au/def/sample-preparation-methods> ;
.

smprep:disaggregate
    a skos:Concept ;
    dcterms:provenance "Compiled by the Geological Survey of Queensland" ;
    rdfs:isDefinedBy <https://linked.data.gov.au/def/sample-preparation-methods> ;
    skos:definition "To separate into component parts"@en ;
    skos:inScheme <https://linked.data.gov.au/def/sample-preparation-methods> ;
    skos:prefLabel "Disaggregate"@en ;
    skos:topConceptOf <https://linked.data.gov.au/def/sample-preparation-methods> ;
.

smprep:dissolve
    a skos:Concept ;
    dcterms:provenance "Compiled by the Geological Survey of Queensland" ;
    rdfs:isDefinedBy <https://linked.data.gov.au/def/sample-preparation-methods> ;
    skos:definition "The process of dissolving a material in a solvent."@en ;
    skos:inScheme <https://linked.data.gov.au/def/sample-preparation-methods> ;
    skos:prefLabel "Dissolve"@en ;
    skos:topConceptOf <https://linked.data.gov.au/def/sample-preparation-methods> ;
.

smprep:distill
    a skos:Concept ;
    dcterms:provenance "Compiled by the Geological Survey of Queensland" ;
    rdfs:isDefinedBy <https://linked.data.gov.au/def/sample-preparation-methods> ;
    skos:definition "The action of purifying a liquid by a process of heating and cooling."@en ;
    skos:inScheme <https://linked.data.gov.au/def/sample-preparation-methods> ;
    skos:prefLabel "Distill"@en ;
    skos:topConceptOf <https://linked.data.gov.au/def/sample-preparation-methods> ;
.

smprep:extract
    a skos:Concept ;
    dcterms:provenance "Compiled by the Geological Survey of Queensland" ;
    rdfs:isDefinedBy <https://linked.data.gov.au/def/sample-preparation-methods> ;
    skos:definition "A separation process consisting in the separation of a substance from a matrix. Common examples include liquid-liquid extraction, and solid phase extraction."@en ;
    skos:inScheme <https://linked.data.gov.au/def/sample-preparation-methods> ;
    skos:prefLabel "Extract"@en ;
    skos:topConceptOf <https://linked.data.gov.au/def/sample-preparation-methods> ;
.

smprep:filter
    a skos:Concept ;
    dcterms:provenance "Compiled by the Geological Survey of Queensland" ;
    rdfs:isDefinedBy <https://linked.data.gov.au/def/sample-preparation-methods> ;
    skos:definition "An operation that separates solid matter and fluid from a mixture with a filter medium that has a complex structure through which only the fluid can pass."@en ;
    skos:inScheme <https://linked.data.gov.au/def/sample-preparation-methods> ;
    skos:prefLabel "Filter"@en ;
    skos:topConceptOf <https://linked.data.gov.au/def/sample-preparation-methods> ;
.

smprep:freeze
    a skos:Concept ;
    dcterms:provenance "Compiled by the Geological Survey of Queensland" ;
    rdfs:isDefinedBy <https://linked.data.gov.au/def/sample-preparation-methods> ;
    skos:altLabel "Solidify"@en ;
    skos:definition "To change a liquid to a solid. Typically through decreasing temperature or increasing pressure."@en ;
    skos:inScheme <https://linked.data.gov.au/def/sample-preparation-methods> ;
    skos:prefLabel "Freeze"@en ;
    skos:topConceptOf <https://linked.data.gov.au/def/sample-preparation-methods> ;
.

smprep:gravity-concentrate
    a skos:Concept ;
    dcterms:provenance "Compiled by the Geological Survey of Queensland" ;
    rdfs:isDefinedBy <https://linked.data.gov.au/def/sample-preparation-methods> ;
    skos:altLabel
        "Float-and-Sink Separation"@en ,
        "Gravity Separation"@en ,
        "Sink-and-Float Separation"@en ;
    skos:broader smprep:concentrate ;
    skos:definition "Preparation by removing or reducing the diluting material through the action of gravity by utilising density difference between the target material and host material."@en ;
    skos:inScheme <https://linked.data.gov.au/def/sample-preparation-methods> ;
    skos:prefLabel "Gravity Concentrate"@en ;
.

smprep:grind
    a skos:Concept ;
    dcterms:provenance "Compiled by the Geological Survey of Queensland" ;
    rdfs:isDefinedBy <https://linked.data.gov.au/def/sample-preparation-methods> ;
    skos:definition "Reduce of material to small particles or powder by crushing it."@en ;
    skos:inScheme <https://linked.data.gov.au/def/sample-preparation-methods> ;
    skos:prefLabel "Grind"@en ;
    skos:topConceptOf <https://linked.data.gov.au/def/sample-preparation-methods> ;
.

smprep:hydrate
    a skos:Concept ;
    dcterms:provenance "Compiled by the Geological Survey of Queensland" ;
    rdfs:isDefinedBy <https://linked.data.gov.au/def/sample-preparation-methods> ;
    skos:altLabel "Wetting"@en ;
    skos:definition "The addition of water to a solid sample."@en ;
    skos:inScheme <https://linked.data.gov.au/def/sample-preparation-methods> ;
    skos:prefLabel "Hydrate"@en ;
    skos:topConceptOf <https://linked.data.gov.au/def/sample-preparation-methods> ;
.

smprep:ionise
    a skos:Concept ;
    dcterms:provenance "Compiled by the Geological Survey of Queensland" ;
    rdfs:isDefinedBy <https://linked.data.gov.au/def/sample-preparation-methods> ;
    skos:altLabel "Ionize"@en ;
    skos:definition "To change a gas to a plasma. Typically through decreasing temperature."@en ;
    skos:inScheme <https://linked.data.gov.au/def/sample-preparation-methods> ;
    skos:prefLabel "Ionise"@en ;
    skos:topConceptOf <https://linked.data.gov.au/def/sample-preparation-methods> ;
.

smprep:laser-ablate
    a skos:Concept ;
    dcterms:provenance "Compiled by the Geological Survey of Queensland" ;
    rdfs:isDefinedBy <https://linked.data.gov.au/def/sample-preparation-methods> ;
    skos:definition "Laser ablation is the process of removing material from a solid (or occasionally liquid) surface by irradiating it with a laser beam."@en ;
    skos:inScheme <https://linked.data.gov.au/def/sample-preparation-methods> ;
    skos:prefLabel "Laser Ablate"@en ;
    skos:topConceptOf <https://linked.data.gov.au/def/sample-preparation-methods> ;
.

smprep:mount
    a skos:Concept ;
    dcterms:provenance "Compiled by the Geological Survey of Queensland" ;
    rdfs:isDefinedBy <https://linked.data.gov.au/def/sample-preparation-methods> ;
    skos:definition "To be mounted on or between media in preparation for petroscopy or other observation technique which requires a stable, protected sample."@en ;
    skos:inScheme <https://linked.data.gov.au/def/sample-preparation-methods> ;
    skos:prefLabel "Mount"@en ;
    skos:topConceptOf <https://linked.data.gov.au/def/sample-preparation-methods> ;
.

smprep:partial-cut
    a skos:Concept ;
    dcterms:provenance "Compiled by the Geological Survey of Queensland" ;
    rdfs:isDefinedBy <https://linked.data.gov.au/def/sample-preparation-methods> ;
    skos:broader smprep:cut ;
    skos:definition "Prepartion by bifurcating any number of times to produce fresh faces or a smaller overall sample, but where un-cut surfaces remain on the sample material."@en ;
    skos:inScheme <https://linked.data.gov.au/def/sample-preparation-methods> ;
    skos:prefLabel "Partial Cut"@en ;
.

smprep:precipitate
    a skos:Concept ;
    dcterms:provenance "Compiled by the Geological Survey of Queensland" ;
    rdfs:isDefinedBy <https://linked.data.gov.au/def/sample-preparation-methods> ;
    skos:definition "The process of precipitating a material out of a solvent."@en ;
    skos:inScheme <https://linked.data.gov.au/def/sample-preparation-methods> ;
    skos:prefLabel "Precipitate"@en ;
    skos:topConceptOf <https://linked.data.gov.au/def/sample-preparation-methods> ;
.

smprep:react
    a skos:Concept ;
    dcterms:provenance "Compiled by the Geological Survey of Queensland" ;
    rdfs:isDefinedBy <https://linked.data.gov.au/def/sample-preparation-methods> ;
    skos:definition "To change the chemical state of a sample by combination with a reagent."@en ;
    skos:inScheme <https://linked.data.gov.au/def/sample-preparation-methods> ;
    skos:prefLabel "React"@en ;
    skos:topConceptOf <https://linked.data.gov.au/def/sample-preparation-methods> ;
.

smprep:recombine
    a skos:Concept ;
    dcterms:provenance "Compiled by the Geological Survey of Queensland" ;
    rdfs:isDefinedBy <https://linked.data.gov.au/def/sample-preparation-methods> ;
    skos:definition "To change a gas to a plasma. Typically through increasing temperature."@en ;
    skos:inScheme <https://linked.data.gov.au/def/sample-preparation-methods> ;
    skos:prefLabel "Recombine"@en ;
    skos:topConceptOf <https://linked.data.gov.au/def/sample-preparation-methods> ;
.

smprep:sieve
    a skos:Concept ;
    dcterms:provenance "Compiled by the Geological Survey of Queensland" ;
    rdfs:isDefinedBy <https://linked.data.gov.au/def/sample-preparation-methods> ;
    skos:definition "Material characterised by size fractionation through a screen or series of screens."@en ;
    skos:inScheme <https://linked.data.gov.au/def/sample-preparation-methods> ;
    skos:prefLabel "Sieve"@en ;
    skos:topConceptOf <https://linked.data.gov.au/def/sample-preparation-methods> ;
.

smprep:smelt
    a skos:Concept ;
    dcterms:provenance "Compiled by the Geological Survey of Queensland" ;
    rdfs:isDefinedBy <https://linked.data.gov.au/def/sample-preparation-methods> ;
    skos:broader smprep:heat ;
    skos:definition "The process of applying heat to ore in order to extract a base metal. Smelting uses heat and a chemical reducing agent to decompose the ore by separating other elements as gases or slag from the ore and resulting in a purified metal base."@en ;
    skos:inScheme <https://linked.data.gov.au/def/sample-preparation-methods> ;
    skos:prefLabel "Smelt"@en ;
.

smprep:smelt-byproduct
    a skos:Concept ;
    dcterms:provenance "Compiled by the Geological Survey of Queensland" ;
    rdfs:isDefinedBy <https://linked.data.gov.au/def/sample-preparation-methods> ;
    skos:altLabel
        "Smelt Waste"@en ,
        "Smelting Waste"@en ;
    skos:broader smprep:heat ;
    skos:definition "The by-product pathway parallel to a smelting process that generates waste material or by-products."@en ;
    skos:inScheme <https://linked.data.gov.au/def/sample-preparation-methods> ;
    skos:prefLabel "Smelt By-product"@en ;
.

smprep:sublimate
    a skos:Concept ;
    dcterms:provenance "Compiled by the Geological Survey of Queensland" ;
    rdfs:isDefinedBy <https://linked.data.gov.au/def/sample-preparation-methods> ;
    skos:definition "To change a solid to a gas. Typically through increasing temperature or decreasing pressure."@en ;
    skos:inScheme <https://linked.data.gov.au/def/sample-preparation-methods> ;
    skos:prefLabel "Sublimate"@en ;
    skos:topConceptOf <https://linked.data.gov.au/def/sample-preparation-methods> ;
.

smprep:thermal-treatment
    a skos:Concept ;
    dcterms:provenance "Compiled by the Geological Survey of Queensland" ;
    rdfs:isDefinedBy <https://linked.data.gov.au/def/sample-preparation-methods> ;
    skos:altLabel
        "Bake"@en ,
        "Baking"@en ,
        "Calcination"@en ;
    skos:broader smprep:heat ;
    skos:definition "The process of applying thermal radiation to a material in order to chemically alter or oxidise it."@en ;
    skos:inScheme <https://linked.data.gov.au/def/sample-preparation-methods> ;
    skos:prefLabel "Thermal treatment"@en ;
.

smprep:vaporise
    a skos:Concept ;
    dcterms:provenance "Compiled by the Geological Survey of Queensland" ;
    rdfs:isDefinedBy <https://linked.data.gov.au/def/sample-preparation-methods> ;
    skos:altLabel
        "Boil"@en ,
        "Vaporize"@en ;
    skos:definition "To change a liquid to a gas. Typically through increasing temperature or decreasing pressure."@en ;
    skos:inScheme <https://linked.data.gov.au/def/sample-preparation-methods> ;
    skos:prefLabel "Vaporise"@en ;
    skos:topConceptOf <https://linked.data.gov.au/def/sample-preparation-methods> ;
.

smprep:beneficiate
    a skos:Concept ;
    dcterms:provenance "Compiled by the Geological Survey of Queensland" ;
    rdfs:isDefinedBy <https://linked.data.gov.au/def/sample-preparation-methods> ;
    owl:hasPart
        smprep:concentrate ,
        smprep:crush ,
        smprep:wash ;
    skos:definition "A composite process that may include any combination of washing, crushing, and concentrating"@en ;
    skos:inScheme <https://linked.data.gov.au/def/sample-preparation-methods> ;
    skos:prefLabel "Beneficiate"@en ;
    skos:topConceptOf <https://linked.data.gov.au/def/sample-preparation-methods> ;
.

smprep:crush-sort
    a skos:Concept ;
    dcterms:provenance "Compiled by the Geological Survey of Queensland" ;
    rdfs:isDefinedBy <https://linked.data.gov.au/def/sample-preparation-methods> ;
    owl:hasPart
        smprep:crush ,
        smprep:sort ;
    skos:definition "A composite process of deformation or pulverization of material by compressing forcefully (crushing) followed by separation of material components based on a physical property such as size or density (sort)."@en ;
    skos:inScheme <https://linked.data.gov.au/def/sample-preparation-methods> ;
    skos:prefLabel "Crush and Sort"@en ;
    skos:topConceptOf <https://linked.data.gov.au/def/sample-preparation-methods> ;
.

smprep:electrolysis
    a skos:Concept ;
    dcterms:provenance "Compiled by the Geological Survey of Queensland" ;
    rdfs:isDefinedBy <https://linked.data.gov.au/def/sample-preparation-methods> ;
    skos:definition "A technique that uses direct electric current to drive an otherwise non-spontaneous chemical reaction. Electrolysis is commercially important as a stage in the separation of elements from naturally occurring sources such as ores using an electrolytic cell."@en ;
    skos:inScheme <https://linked.data.gov.au/def/sample-preparation-methods> ;
    skos:prefLabel "Electrolysis"@en ;
    skos:topConceptOf <https://linked.data.gov.au/def/sample-preparation-methods> ;
.

smprep:refine
    a skos:Concept ;
    dcterms:provenance "Compiled by the Geological Survey of Queensland" ;
    rdfs:isDefinedBy <https://linked.data.gov.au/def/sample-preparation-methods> ;
    owl:hasPart
        smprep:cupellation ,
        smprep:electrolysis ,
        smprep:melt ,
        smprep:thermal-treatment ;
    skos:definition "A group of post-primary process in resource processing such as electrolysis, cupellation, pyrometallurgical reactions."@en ;
    skos:inScheme <https://linked.data.gov.au/def/sample-preparation-methods> ;
    skos:prefLabel "Refine"@en ;
    skos:topConceptOf <https://linked.data.gov.au/def/sample-preparation-methods> ;
.

smprep:refining-byproduct
    a skos:Concept ;
    dcterms:provenance "Compiled by the Geological Survey of Queensland" ;
    rdfs:isDefinedBy <https://linked.data.gov.au/def/sample-preparation-methods> ;
    skos:altLabel "Refining Waste"@en ;
    skos:definition "The by-product pathway parallel to a refining process that generates waste material or by-products."@en ;
    skos:inScheme <https://linked.data.gov.au/def/sample-preparation-methods> ;
    skos:prefLabel "Refining by-product"@en ;
    skos:topConceptOf <https://linked.data.gov.au/def/sample-preparation-methods> ;
.

smprep:rough-extract
    a skos:Concept ;
    dcterms:provenance "Compiled by the Geological Survey of Queensland" ;
    rdfs:isDefinedBy <https://linked.data.gov.au/def/sample-preparation-methods> ;
    skos:definition "To extract gemstones, typically opal, as extracted from-ground or after the agitation process of washing and tumbling, but without processing by apidary equipment."@en ;
    skos:inScheme <https://linked.data.gov.au/def/sample-preparation-methods> ;
    skos:prefLabel "Rough Extract"@en ;
    skos:topConceptOf <https://linked.data.gov.au/def/sample-preparation-methods> ;
.

smprep:sort
    a skos:Concept ;
    dcterms:provenance "Compiled by the Geological Survey of Queensland" ;
    rdfs:isDefinedBy <https://linked.data.gov.au/def/sample-preparation-methods> ;
    skos:definition "The separation of material components based on a physical property such as size or density (sort)"@en ;
    skos:inScheme <https://linked.data.gov.au/def/sample-preparation-methods> ;
    skos:prefLabel "Sort"@en ;
    skos:topConceptOf <https://linked.data.gov.au/def/sample-preparation-methods> ;
.

smprep:unprocessed
    a skos:Concept ;
    dcterms:provenance "Compiled by the Geological Survey of Queensland" ;
    rdfs:isDefinedBy <https://linked.data.gov.au/def/sample-preparation-methods> ;
    skos:altLabel
        "N/A"@en ,
        "Not Applicable"@en ,
        "Unprocessed"@en ;
    skos:definition "An explicit indication that a sample material was not processed between two states. For example where a raw material requires no processing to be considered a saleable product."@en ;
    skos:inScheme <https://linked.data.gov.au/def/sample-preparation-methods> ;
    skos:prefLabel "No Processing"@en ;
    skos:topConceptOf <https://linked.data.gov.au/def/sample-preparation-methods> ;
.

smprep:unspecified
    a skos:Concept ;
    dcterms:provenance "Compiled by the Geological Survey of Queensland" ;
    rdfs:isDefinedBy <https://linked.data.gov.au/def/sample-preparation-methods> ;
    skos:altLabel "Unknown"@en ;
    skos:definition "Where a process or group of processes has been performed but specific details have not been recorded or are not available."@en ;
    skos:inScheme <https://linked.data.gov.au/def/sample-preparation-methods> ;
    skos:prefLabel "Unspecified"@en ;
    skos:topConceptOf <https://linked.data.gov.au/def/sample-preparation-methods> ;
.

smprep:wash
    a skos:Concept ;
    dcterms:provenance "Compiled by the Geological Survey of Queensland" ;
    rdfs:isDefinedBy <https://linked.data.gov.au/def/sample-preparation-methods> ;
    skos:definition "To mix with water and/or chemicals and physically agitate to remove impurities."@en ;
    skos:inScheme <https://linked.data.gov.au/def/sample-preparation-methods> ;
    skos:prefLabel "Wash"@en ;
    skos:topConceptOf <https://linked.data.gov.au/def/sample-preparation-methods> ;
.

<https://linked.data.gov.au/org/gsq>
    a sdo:Organization ;
    sdo:name "Geological Survey of Queensland" ;
    sdo:url "http://www.business.qld.gov.au/industries/mining-energy-water/resources/geoscience-information/gsq"^^xsd:anyURI ;
.

smprep:crush
    a skos:Concept ;
    dcterms:provenance "Compiled by the Geological Survey of Queensland" ;
    rdfs:isDefinedBy <https://linked.data.gov.au/def/sample-preparation-methods> ;
    skos:definition "The deformation or pulverization of material by compressing forcefully."@en ;
    skos:inScheme <https://linked.data.gov.au/def/sample-preparation-methods> ;
    skos:prefLabel "Crush"@en ;
    skos:topConceptOf <https://linked.data.gov.au/def/sample-preparation-methods> ;
.

smprep:cut
    a skos:Concept ;
    dcterms:provenance "Compiled by the Geological Survey of Queensland" ;
    rdfs:isDefinedBy <https://linked.data.gov.au/def/sample-preparation-methods> ;
    skos:definition "Prepartion by bifurcating any number of times to produce fresh faces or a smaller overall sample."@en ;
    skos:inScheme <https://linked.data.gov.au/def/sample-preparation-methods> ;
    skos:prefLabel "Cut"@en ;
    skos:topConceptOf <https://linked.data.gov.au/def/sample-preparation-methods> ;
.

smprep:melt
    a skos:Concept ;
    dcterms:provenance "Compiled by the Geological Survey of Queensland" ;
    rdfs:isDefinedBy <https://linked.data.gov.au/def/sample-preparation-methods> ;
    skos:definition "To change a solid to a liquid. Typically through increasing temperature or decreasing pressure."@en ;
    skos:inScheme <https://linked.data.gov.au/def/sample-preparation-methods> ;
    skos:prefLabel "Melt"@en ;
    skos:topConceptOf <https://linked.data.gov.au/def/sample-preparation-methods> ;
.

smprep:concentrate
    a skos:Concept ;
    dcterms:provenance "Compiled by the Geological Survey of Queensland" ;
    rdfs:isDefinedBy <https://linked.data.gov.au/def/sample-preparation-methods> ;
    skos:definition "Preparation by removing or reducing the diluting agent(s) or material."@en ;
    skos:inScheme <https://linked.data.gov.au/def/sample-preparation-methods> ;
    skos:prefLabel "Concentrate"@en ;
    skos:topConceptOf <https://linked.data.gov.au/def/sample-preparation-methods> ;
.

smprep:heat
    a skos:Concept ;
    dcterms:provenance "Compiled by the Geological Survey of Queensland" ;
    rdfs:isDefinedBy <https://linked.data.gov.au/def/sample-preparation-methods> ;
    skos:altLabel "Heating"@en ;
    skos:definition "The process of applying thermal radiation to a material in order to raise its surface and or internal temperature."@en ;
    skos:inScheme <https://linked.data.gov.au/def/sample-preparation-methods> ;
    skos:prefLabel "Heat"@en ;
    skos:topConceptOf <https://linked.data.gov.au/def/sample-preparation-methods> ;
.

<https://linked.data.gov.au/def/sample-preparation-methods>
    a
        owl:Ontology ,
        skos:ConceptScheme ;
    dcterms:created "2020-02-07"^^xsd:date ;
    dcterms:creator <https://linked.data.gov.au/org/gsq> ;
    dcterms:modified "2022-02-23"^^xsd:date ;
    dcterms:provenance "Compiled by the Geological Survey of Queensland" ;
    dcterms:publisher <https://linked.data.gov.au/org/gsq> ;
    skos:definition "The methods used to prepare samples for analyses."@en ;
    skos:hasTopConcept
        smprep:acidify ,
        smprep:aggregate ,
        smprep:beneficiate ,
        smprep:chelate ,
        smprep:compress ,
        smprep:concentrate ,
        smprep:condense ,
        smprep:cool ,
        smprep:crush ,
        smprep:crush-sort ,
        smprep:cut ,
        smprep:deacidify ,
        smprep:decompress ,
        smprep:deposit ,
        smprep:dessicate ,
        smprep:dilute ,
        smprep:disaggregate ,
        smprep:dissolve ,
        smprep:distill ,
        smprep:electrolysis ,
        smprep:extract ,
        smprep:filter ,
        smprep:freeze ,
        smprep:grind ,
        smprep:heat ,
        smprep:hydrate ,
        smprep:ionise ,
        smprep:laser-ablate ,
        smprep:melt ,
        smprep:mount ,
        smprep:precipitate ,
        smprep:react ,
        smprep:recombine ,
        smprep:refine ,
        smprep:refining-byproduct ,
        smprep:rough-extract ,
        smprep:sieve ,
        smprep:sort ,
        smprep:sublimate ,
        smprep:unprocessed ,
        smprep:unspecified ,
        smprep:vaporise ,
        smprep:wash ;
    skos:prefLabel "Sample Preparation Methods"@en ;
.

