@prefix smrl: <http://linked.data.gov.au/def/sample-relationship/> .
@prefix dcterms: <http://purl.org/dc/terms/> .
@prefix owl: <http://www.w3.org/2002/07/owl#> .
@prefix rdfs: <http://www.w3.org/2000/01/rdf-schema#> .
@prefix sdo: <http://schema.org/> .
@prefix skos: <http://www.w3.org/2004/02/skos/core#> .
@prefix sosa: <http://www.w3.org/ns/sosa/> .
@prefix xsd: <http://www.w3.org/2001/XMLSchema#> .

<http://linked.data.gov.au/def/sample-relationship> a owl:Ontology , skos:ConceptScheme ;
    dcterms:created "2020-03-24"^^xsd:date ;
    dcterms:creator <http://linked.data.gov.au/org/gsq> ;
    dcterms:modified "2022-01-04"^^xsd:date ;
    dcterms:publisher <http://linked.data.gov.au/org/gsq> ;
    dcterms:provenance "Source information from http://www.w3.org/TR/vocab-ssn/#Sample_Relations and the SOSA Extensions ontology, modified by the Geological Survey of Queensland." ;
    skos:definition """Relationships between Samples. This vocabulary is derived from the SOSA Ontology and the SOSA Extensions Ontology where the Samples are defined by the class sosa:Sample and the relationships are OWL objectProperties. It reuses the original ontology URIs directly and retains the relationship's non-SKSO properties too so it is a SKOS+ ontology (SKOS + other things)."""@en ;
    skos:hasTopConcept
        #sosa:hasSample ,
        smrl:isAggregateOf ,
        sosa:isSampleOf ,
        sosa:hasOriginalSample ;
    skos:prefLabel "Sample Relationship"@en .

<http://linked.data.gov.au/org/gsq>
    a sdo:Organization ;
    sdo:name "Geological Survey of Queensland" ;
    sdo:url "http://www.business.qld.gov.au/industries/mining-energy-water/resources/geoscience-information/gsq"^^xsd:anyURI .

#sosa:hasSample
#    a owl:ObjectProperty , skos:Concept ;
#    skos:prefLabel "has sample"@en ;
#    skos:definition "Relation between a subject and a sample dervied from it."@en ;
#    sdo:domainIncludes sosa:FeatureOfInterest ;
#    sdo:rangeIncludes sosa:Sample ;
#    owl:inverseOf sosa:isSampleOf ;
#    rdfs:isDefinedBy sosa: ;
#    skos:inScheme <http://linked.data.gov.au/def/sample-relationship> ;
#    skos:topConceptOf <http://linked.data.gov.au/def/sample-relationship> .

smrl:isAggregateOf
    a skos:Concept ;
    skos:prefLabel "is aggregate of"@en ;
    skos:definition "Relation from a Sample to an entity that it was dervied from, where multiple sources have been aggregated into a composite sample."@en ;
    sdo:domainIncludes sosa:Sample ;
    rdfs:isDefinedBy <http://linked.data.gov.au/def/sample-relationship> ;
    skos:inScheme <http://linked.data.gov.au/def/sample-relationship> ;
    skos:topConceptOf <http://linked.data.gov.au/def/sample-relationship> .

sosa:isSampleOf
    a owl:ObjectProperty , skos:Concept ;
    skos:prefLabel "is sample of"@en ;
    skos:definition "Relation from a Sample to the entity that it was dervied from."@en ;
    sdo:domainIncludes sosa:Sample ;
    sdo:rangeIncludes sosa:FeatureOfInterest ;
    owl:inverseOf sosa:hasSample ;
    rdfs:isDefinedBy sosa: ;
    skos:inScheme <http://linked.data.gov.au/def/sample-relationship> ;
    skos:topConceptOf <http://linked.data.gov.au/def/sample-relationship> .

sosa:hasOriginalSample
    a owl:ObjectProperty , skos:Concept ;
    skos:prefLabel "has original sample"@en ;
    sdo:domainIncludes sosa:Sample ;
    sdo:rangeIncludes sosa:Sample ;
    skos:definition "A link from the subject sample to the original sample of interest through a chain of isSampleOf relations."@en ;
    rdfs:domain sosa:Sample ;
    rdfs:isDefinedBy sosa: ;
    rdfs:range sosa:Sample ;
    skos:inScheme <http://linked.data.gov.au/def/sample-relationship> ;
    skos:topConceptOf <http://linked.data.gov.au/def/sample-relationship> .

