PREFIX dcterms: <http://purl.org/dc/terms/>
PREFIX owl: <http://www.w3.org/2002/07/owl#>
PREFIX rdfs: <http://www.w3.org/2000/01/rdf-schema#>
PREFIX sdo: <http://schema.org/>
PREFIX skos: <http://www.w3.org/2004/02/skos/core#>
PREFIX smlcst: <http://linked.data.gov.au/def/sample-location-status/>
PREFIX xsd: <http://www.w3.org/2001/XMLSchema#>

smlcst:collected
    a skos:Concept ;
    dcterms:provenance "Compiled by the Geological Survey of Queensland" ;
    rdfs:isDefinedBy <http://linked.data.gov.au/def/sample-location-status> ;
    skos:definition "Sample has been collected from a sampling location and is in temporary storage prior to transfer to permanent or semi-permanent storage"@en ;
    skos:inScheme <http://linked.data.gov.au/def/sample-location-status> ;
    skos:prefLabel "Collected"@en ;
    skos:topConceptOf <http://linked.data.gov.au/def/sample-location-status> ;
.

smlcst:in-storage
    a skos:Concept ;
    dcterms:provenance "Compiled by the Geological Survey of Queensland" ;
    rdfs:isDefinedBy <http://linked.data.gov.au/def/sample-location-status> ;
    skos:altLabel "Static"@en ;
    skos:definition "Held at a storage location in an archived state."@en ;
    skos:inScheme <http://linked.data.gov.au/def/sample-location-status> ;
    skos:prefLabel "In Storage"@en ;
    skos:topConceptOf <http://linked.data.gov.au/def/sample-location-status> ;
.

smlcst:in-transit
    a skos:Concept ;
    dcterms:provenance "Compiled by the Geological Survey of Queensland" ;
    rdfs:isDefinedBy <http://linked.data.gov.au/def/sample-location-status> ;
    skos:definition "In transit between locations."@en ;
    skos:inScheme <http://linked.data.gov.au/def/sample-location-status> ;
    skos:prefLabel "In transit"@en ;
    skos:topConceptOf <http://linked.data.gov.au/def/sample-location-status> ;
.

smlcst:lost
    a skos:Concept ;
    dcterms:provenance "Compiled by the Geological Survey of Queensland" ;
    rdfs:isDefinedBy <http://linked.data.gov.au/def/sample-location-status> ;
    skos:definition "Location of sample is not known"@en ;
    skos:inScheme <http://linked.data.gov.au/def/sample-location-status> ;
    skos:prefLabel "Lost"@en ;
    skos:topConceptOf <http://linked.data.gov.au/def/sample-location-status> ;
.

smlcst:on-display
    a skos:Concept ;
    dcterms:provenance "Compiled by the Geological Survey of Queensland" ;
    rdfs:isDefinedBy <http://linked.data.gov.au/def/sample-location-status> ;
    skos:definition "Held in a storage facility, museum, or other location for display and/or analysis."@en ;
    skos:inScheme <http://linked.data.gov.au/def/sample-location-status> ;
    skos:prefLabel "On Display"@en ;
    skos:topConceptOf <http://linked.data.gov.au/def/sample-location-status> ;
.

smlcst:processing
    a skos:Concept ;
    dcterms:provenance "Compiled by the Geological Survey of Queensland" ;
    rdfs:isDefinedBy <http://linked.data.gov.au/def/sample-location-status> ;
    skos:altLabel
        "Analysis"@en ,
        "Laboratory"@en ;
    skos:definition "The sample is at a laboratory, university, or other facility external to its registered storage facility undergoing processing or analysis."@en ;
    skos:inScheme <http://linked.data.gov.au/def/sample-location-status> ;
    skos:prefLabel "Processing"@en ;
    skos:topConceptOf <http://linked.data.gov.au/def/sample-location-status> ;
.

<http://linked.data.gov.au/org/gsq>
    a sdo:Organization ;
    sdo:name "Geological Survey of Queensland" ;
    sdo:url "http://www.business.qld.gov.au/industries/mining-energy-water/resources/geoscience-information/gsq"^^xsd:anyURI ;
.

<http://linked.data.gov.au/def/sample-location-status>
    a
        owl:Ontology ,
        skos:ConceptScheme ;
    dcterms:created "2020-02-07T13:27:05"^^xsd:dateTime ;
    dcterms:creator <http://linked.data.gov.au/org/gsq> ;
    dcterms:modified "2020-02-08T11:42:48"^^xsd:dateTime ;
    dcterms:provenance "Compiled by the Geological Survey of Queensland" ;
    dcterms:publisher <http://linked.data.gov.au/org/gsq> ;
    skos:definition "The status of a sample with respect to its location."@en ;
    skos:hasTopConcept
        smlcst:collected ,
        smlcst:in-storage ,
        smlcst:in-transit ,
        smlcst:lost ,
        smlcst:on-display ,
        smlcst:processing ;
    skos:prefLabel "Sample Location Status"@en ;
.

