@prefix dc: <http://purl.org/dc/elements/1.1/> .
@prefix dcterms: <http://purl.org/dc/terms/> .
@prefix dcterms: <http://purl.org/dc/terms/> .
@prefix owl: <http://www.w3.org/2002/07/owl#> .
@prefix sdo: <http://schema.org/> .
@prefix skos: <http://www.w3.org/2004/02/skos/core#> .
@prefix svydt: <http://linked.data.gov.au/def/survey-detail-type/> .
@prefix rdfs: <http://www.w3.org/2000/01/rdf-schema#> .
@prefix xsd: <http://www.w3.org/2001/XMLSchema#> .

<http://linked.data.gov.au/def/survey-detail-type> a owl:Ontology,
        skos:ConceptScheme ;
    dcterms:created "2020-03-30"^^xsd:date ;
    dcterms:creator <http://linked.data.gov.au/org/gsq> ;
    dcterms:modified "2022-02-04"^^xsd:date ;
    dcterms:publisher <http://linked.data.gov.au/org/gsq> ;
    skos:definition "Miscellaneous Survey Details."@en ;
    skos:hasTopConcept svydt:active-period,
        svydt:ag-survey-type,
        svydt:comments,
        svydt:full-time-employees,
        svydt:full-time-contractors,
        svydt:funding-program,
        svydt:historic-tenure,
        svydt:historic-title,
        svydt:interval-m,
        svydt:job-number,
        svydt:line-direction-degrees,
        svydt:locality,
        svydt:report-period-freight-cost,
        svydt:survey-height-m,
        svydt:survey-line,
        svydt:tie-interval-m,
        svydt:tie-line-direction-degrees,
        svydt:total-line-kilometres,
        svydt:total-stations,
        svydt:vessel-name ;
    skos:prefLabel "Survey Detail Type"@en .

<http://linked.data.gov.au/org/gsq> a sdo:Organization ;
    sdo:name "Geological Survey of Queensland" ;
    sdo:url "https://www.business.qld.gov.au/industries/mining-energy-water/resources/geoscience-information/gsq"^^xsd:anyURI .

svydt:ag-survey-type a skos:Concept ;
    skos:definition "Airborne geophysical survey type (exploration, government, open range, multi-client or experimental)"@en ;
    rdfs:isDefinedBy <http://linked.data.gov.au/def/survey-detail-type> ;
    skos:inScheme <http://linked.data.gov.au/def/survey-detail-type> ;
    skos:prefLabel "AG Survey Type"@en ;
    skos:topConceptOf <http://linked.data.gov.au/def/survey-detail-type> .

svydt:total-stations a skos:Concept ;
    skos:definition "Number of stations included in survey"@en ;
    rdfs:isDefinedBy <http://linked.data.gov.au/def/survey-detail-type> ;
    skos:inScheme <http://linked.data.gov.au/def/survey-detail-type> ;
    skos:prefLabel "Total Stations"@en ;
    skos:topConceptOf <http://linked.data.gov.au/def/survey-detail-type> .

svydt:full-time-employees a skos:Concept ;
    skos:altLabel "FTE Employees"@en,
        "Full-time equivalent employees"@en,
        "Full-Time (FTE) Equivalent Employees"@en ;
    skos:definition "The full-time equivalent (FTE) number of employees working on a project throughout the reporting period."@en ;
    rdfs:isDefinedBy <http://linked.data.gov.au/def/survey-detail-type> ;
    skos:inScheme <http://linked.data.gov.au/def/survey-detail-type> ;
    skos:prefLabel "Full-Time Equivalent Employees"@en ;
    skos:topConceptOf <http://linked.data.gov.au/def/survey-detail-type> .

svydt:full-time-contractors a skos:Concept ;
    skos:altLabel "FTE Contractors"@en,
        "Full-time equivalent contractors"@en,
        "Full-Time (FTE) Equivalent Contractors"@en ;
    skos:definition "The full-time equivalent (FTE) number of contract workers (contractors) working on a project throughout the reporting period."@en ;
    rdfs:isDefinedBy <http://linked.data.gov.au/def/survey-detail-type> ;
    skos:inScheme <http://linked.data.gov.au/def/survey-detail-type> ;
    skos:prefLabel "Full-Time Equivalent Contractors"@en ;
    skos:topConceptOf <http://linked.data.gov.au/def/survey-detail-type> .

svydt:historic-tenure a skos:Concept ;
    skos:altLabel "Historic Permit"@en,
        "Legacy Permit"@en ,
        "Legacy Tenure"@en,
        "Previous System Tenure"@en ;
    skos:definition "A legacy tenure or permit identifier that is not in current usage."@en ;
    rdfs:isDefinedBy <http://linked.data.gov.au/def/survey-detail-type> ;
    skos:inScheme <http://linked.data.gov.au/def/survey-detail-type> ;
    skos:prefLabel "Historic Tenure"@en ;
    skos:topConceptOf <http://linked.data.gov.au/def/survey-detail-type> .

svydt:historic-title a skos:Concept ;
    skos:altLabel "Legacy Title"@en,
        "Former Plan Number"@en ;
    skos:definition "A previous title or reference to the survey or document that has been edited, amended, or replaced."@en ;
    rdfs:isDefinedBy <http://linked.data.gov.au/def/survey-detail-type> ;
    skos:inScheme <http://linked.data.gov.au/def/survey-detail-type> ;
    skos:prefLabel "Historic Title"@en ;
    skos:topConceptOf <http://linked.data.gov.au/def/survey-detail-type> .

svydt:locality a skos:Concept ;
    skos:definition "A geographic subdivision or district used in rural and regional Australia. Localities are commonly based on a local feature or township, but some occurrences may be subjectively named."@en ;
    rdfs:isDefinedBy <http://linked.data.gov.au/def/survey-detail-type> ;
    skos:inScheme <http://linked.data.gov.au/def/survey-detail-type> ;
    skos:prefLabel "Locality"@en ;
    skos:topConceptOf <http://linked.data.gov.au/def/survey-detail-type> .

svydt:line-direction-degrees a skos:Concept ;
    skos:definition "Mean survey line direction (bearing) from true north.  Values between 000-359 degrees"@en ;
    rdfs:isDefinedBy <http://linked.data.gov.au/def/survey-detail-type> ;
    skos:inScheme <http://linked.data.gov.au/def/survey-detail-type> ;
    skos:prefLabel "Line Direction (degrees)"@en ;
    skos:topConceptOf <http://linked.data.gov.au/def/survey-detail-type> .

svydt:survey-height-m a skos:Concept ;
    skos:altLabel "terrain clearance"@en ;
    skos:definition "Mean survey height above ground surface (values in metres relative to AHD)"@en ;
    rdfs:isDefinedBy <http://linked.data.gov.au/def/survey-detail-type> ;
    skos:inScheme <http://linked.data.gov.au/def/survey-detail-type> ;
    skos:prefLabel "Survey Height (m)"@en ;
    skos:topConceptOf <http://linked.data.gov.au/def/survey-detail-type> .

svydt:survey-line a skos:Concept ;
    skos:definition "List of survey lines (comma deliminated) included in the survey"@en ;
    rdfs:isDefinedBy <http://linked.data.gov.au/def/survey-detail-type> ;
    skos:inScheme <http://linked.data.gov.au/def/survey-detail-type> ;
    skos:prefLabel "Survey Line"@en ;
    skos:topConceptOf <http://linked.data.gov.au/def/survey-detail-type> .

svydt:tie-interval-m a skos:Concept ;
    skos:altLabel "tie line spacing"@en ;
    skos:definition "Mean distance in metres between survey tie lines (if used) in regularly spaced survey"@en ;
    rdfs:isDefinedBy <http://linked.data.gov.au/def/survey-detail-type> ;
    skos:inScheme <http://linked.data.gov.au/def/survey-detail-type> ;
    skos:prefLabel "Tie Interval (m)"@en ;
    skos:topConceptOf <http://linked.data.gov.au/def/survey-detail-type> .

svydt:tie-line-direction-degrees a skos:Concept ;
    skos:definition "Mean survey tie line direction (bearing) from true north (often perpendicular to line direction).  Values between 000-359"@en ;
    rdfs:isDefinedBy <http://linked.data.gov.au/def/survey-detail-type> ;
    skos:inScheme <http://linked.data.gov.au/def/survey-detail-type> ;
    skos:prefLabel "Tie Line Direction (degrees)"@en ;
    skos:topConceptOf <http://linked.data.gov.au/def/survey-detail-type> .

svydt:vessel-name a skos:Concept ;
    skos:definition "Name, or call sign, of survey vessel (plane, helicopter, boat).  Further information on vessel may also be added"@en ;
    rdfs:isDefinedBy <http://linked.data.gov.au/def/survey-detail-type> ;
    skos:inScheme <http://linked.data.gov.au/def/survey-detail-type> ;
    skos:prefLabel "Vessel Name"@en ;
    skos:topConceptOf <http://linked.data.gov.au/def/survey-detail-type> .

svydt:interval-m a skos:Concept ;
    skos:altLabel "line spacing"@en,
        "station spacing"@en ;
    skos:definition "Mean distance in metres between survey lines or stations for a regularly spaced survey"@en ;
    rdfs:isDefinedBy <http://linked.data.gov.au/def/survey-detail-type> ;
    skos:inScheme <http://linked.data.gov.au/def/survey-detail-type> ;
    skos:prefLabel "Interval (m)"@en ;
    skos:topConceptOf <http://linked.data.gov.au/def/survey-detail-type> .

svydt:total-line-kilometres a skos:Concept ;
    skos:definition "Sum of the length of lines contained in the survey in kilometres."@en ;
    rdfs:isDefinedBy <http://linked.data.gov.au/def/survey-detail-type> ;
    skos:inScheme <http://linked.data.gov.au/def/survey-detail-type> ;
    skos:prefLabel "Total Line Kilometres"@en ;
    skos:topConceptOf <http://linked.data.gov.au/def/survey-detail-type> .

svydt:comments a skos:Concept ;
    skos:definition "Free text comments or notes regarding survey"@en ;
    rdfs:isDefinedBy <http://linked.data.gov.au/def/survey-detail-type> ;
    skos:inScheme <http://linked.data.gov.au/def/survey-detail-type> ;
    skos:prefLabel "Comments"@en ;
    skos:topConceptOf <http://linked.data.gov.au/def/survey-detail-type> .

svydt:funding-program a skos:Concept ;
    skos:definition "Government funding program that survey was conducted under"@en ;
    rdfs:isDefinedBy <http://linked.data.gov.au/def/survey-detail-type> ;
    skos:inScheme <http://linked.data.gov.au/def/survey-detail-type> ;
    skos:prefLabel "Funding program"@en ;
    skos:topConceptOf <http://linked.data.gov.au/def/survey-detail-type> .

svydt:job-number a skos:Concept ;
    skos:definition "Survey contractors job number / job identification"@en ;
    rdfs:isDefinedBy <http://linked.data.gov.au/def/survey-detail-type> ;
    skos:inScheme <http://linked.data.gov.au/def/survey-detail-type> ;
    skos:prefLabel "Job Number"@en ;
    skos:topConceptOf <http://linked.data.gov.au/def/survey-detail-type> .

svydt:report-period-freight-cost a skos:Concept ;
    skos:definition "The total freight charged to the reporting mine during the reporting period (AUD)"@en ;
    rdfs:isDefinedBy <http://linked.data.gov.au/def/survey-detail-type> ;
    skos:inScheme <http://linked.data.gov.au/def/survey-detail-type> ;
    skos:prefLabel "Report Period Freight Cost"@en ;
    skos:topConceptOf <http://linked.data.gov.au/def/survey-detail-type> .

svydt:active-period a skos:Concept ;
    skos:definition "The number of days during the reporting period (month) on which production occurred."@en ;
    rdfs:isDefinedBy <http://linked.data.gov.au/def/survey-detail-type> ;
    skos:inScheme <http://linked.data.gov.au/def/survey-detail-type> ;
    skos:prefLabel "Active Period"@en ;
    skos:topConceptOf <http://linked.data.gov.au/def/survey-detail-type> .

svydt:airborne-geophysics a skos:Collection ;
    skos:definition "Additional details that describe Airborne Geophysics surveys."@en ;
    skos:member svydt:ag-survey-type,
        svydt:comments,
        svydt:funding-program,
        svydt:interval-m,
        svydt:job-number,
        svydt:line-direction-degrees,
        svydt:survey-height-m,
        svydt:tie-interval-m,
        svydt:tie-line-direction-degrees,
        svydt:total-line-kilometres,
        svydt:vessel-name ;
    skos:prefLabel "Airborne Geophysics"@en .

svydt:airborne-spectral a skos:Collection ;
    skos:definition "Additional details that describe Airborne Spectral surveys."@en ;
    skos:member svydt:comments,
        svydt:funding-program,
        svydt:interval-m,
        svydt:job-number,
        svydt:line-direction-degrees,
        svydt:survey-height-m,
        svydt:tie-interval-m,
        svydt:tie-line-direction-degrees,
        svydt:total-line-kilometres,
        svydt:vessel-name ;
    skos:prefLabel "Airborne Spectral"@en .

svydt:ground-geophysics a skos:Collection ;
    skos:definition "Additional details that describe Ground Geophysics surveys."@en ;
    skos:member svydt:comments,
        svydt:funding-program,
        svydt:interval-m,
        svydt:job-number,
        svydt:survey-line,
        svydt:total-stations ;
    skos:prefLabel "Ground Geophysics"@en .

svydt:seismic-surveys a skos:Collection ;
    skos:definition "Additional details that describe Seismic Surveys surveys."@en ;
    skos:member svydt:comments,
        svydt:funding-program,
        svydt:job-number,
        svydt:survey-line,
        svydt:total-line-kilometres ;
    skos:prefLabel "Seismic Surveys"@en .

svydt:survey-plans a skos:Collection ;
    skos:definition "Additional details that describe Survey Plans."@en ;
    skos:member svydt:comments,
        svydt:historic-tenure,
        svydt:historic-title,
        svydt:locality ;
    skos:prefLabel "Survey Plans"@en .
