@prefix dcterms: <http://purl.org/dc/terms/> .
@prefix owl: <http://www.w3.org/2002/07/owl#> .
@prefix sdo: <http://schema.org/> .
@prefix skos: <http://www.w3.org/2004/02/skos/core#> .
@prefix trns: <http://linked.data.gov.au/def/transaction-type/> .
@prefix rdfs: <http://www.w3.org/2000/01/rdf-schema#> .
@prefix xsd: <http://www.w3.org/2001/XMLSchema#> .

<http://linked.data.gov.au/def/transaction-type> a owl:Ontology , skos:ConceptScheme ;
    dcterms:created "2022-01-10"^^xsd:date ;
    dcterms:creator <http://linked.data.gov.au/org/gsq> ;
    dcterms:modified "2022-08-24"^^xsd:date ;
    dcterms:publisher <http://linked.data.gov.au/org/gsq> ;
    dcterms:provenance "Compiled by the Geological Survey of Queensland" ;
    skos:definition "The types of transactions between parties as pertains to the provision of goods, materials, and services."@en ;
    skos:hasTopConcept trns:sale,
        trns:purchase,
        trns:transfer-in,
        trns:transfer-out,
        trns:loan,
        trns:borrow,
        trns:exchange ;
    skos:prefLabel "Transaction Type"@en .

<http://linked.data.gov.au/org/gsq> a sdo:Organization ;
    sdo:name "Geological Survey of Queensland" ;
    sdo:url "http://www.business.qld.gov.au/industries/mining-energy-water/resources/geoscience-information/gsq"^^xsd:anyURI .

trns:sale a skos:Concept ;
    skos:topConceptOf <http://linked.data.gov.au/def/transaction-type> ;
    skos:definition "The supply of goods or provision of services from the subject party, in exchange for a currency value. Where the reporting or subject party has sold goods or services to another party. An exchange of goods or services for money"@en ;
    rdfs:isDefinedBy <http://linked.data.gov.au/def/transaction-type> ;
    skos:inScheme <http://linked.data.gov.au/def/transaction-type> ;
    skos:prefLabel "Sale"@en .

trns:purchase a skos:Concept ;
    skos:topConceptOf <http://linked.data.gov.au/def/transaction-type> ;
    skos:definition "A transaction of a currency value from the subject party in exchange for goods or the provision of services. Where the reporting or subject party has received goods or services from another party. An exchange of money for goods or services"@en ;
    rdfs:isDefinedBy <http://linked.data.gov.au/def/transaction-type> ;
    skos:inScheme <http://linked.data.gov.au/def/transaction-type> ;
    skos:prefLabel "Purchase"@en .

trns:purchase-feed a skos:Concept ;
    skos:altLabel "Purchase (Raw)"@en ;
    skos:broader trns:purchase ;
    skos:definition "A type of purchase in which the goods exchanged will undergo further processing or refining by the buyer prior to onward sale. A purchase of good that will contribute to the feedstock to processing by the purchasing entity."@en ;
    rdfs:isDefinedBy <http://linked.data.gov.au/def/transaction-type> ;
    skos:inScheme <http://linked.data.gov.au/def/transaction-type> ;
    skos:prefLabel "Purchase (Feedstock)"@en .

trns:transfer-in a skos:Concept ;
    skos:altLabel "Inward Transfer"@en,
        "Inbound Transfer"@en,
        "Goods Received"@en ;
    skos:hiddenLabel "In"@en ;
    skos:topConceptOf <http://linked.data.gov.au/def/transaction-type> ;
    skos:definition "A transfer of material to the subject party. Where the reporting or subject party has received goods or services from another party, without a financial component to the transaction. Such as where goods have been transferred from a separate part of the same single company."@en ;
    skos:example "Where a mine has recieved raw material from another mine owned by the same company for processing or amalgamated sale"@en ;
    rdfs:isDefinedBy <http://linked.data.gov.au/def/transaction-type> ;
    skos:inScheme <http://linked.data.gov.au/def/transaction-type> ;
    skos:prefLabel "Transfer In"@en .

trns:transfer-out a skos:Concept ;
    skos:altLabel "Outward Transfer"@en,
        "Outbound Transfer"@en,
        "Goods Dispatched"@en ;
    skos:hiddenLabel "Out"@en ;
    skos:topConceptOf <http://linked.data.gov.au/def/transaction-type> ;
    skos:definition "A transfer of material from the subject party. Where the reporting or subject party has sent goods or services to another party, without a financial component to the transaction. Such as where goods have been transferred to a separate part of the same single company."@en ;
    skos:example "Where a mine has sent raw material to another mine owned by the same company for processing or amalgamated sale"@en ;
    rdfs:isDefinedBy <http://linked.data.gov.au/def/transaction-type> ;
    skos:inScheme <http://linked.data.gov.au/def/transaction-type> ;
    skos:prefLabel "Transfer Out"@en .

trns:loan a skos:Concept ;
    skos:topConceptOf <http://linked.data.gov.au/def/transaction-type> ;
    skos:definition "The supply goods with the agreement that the goods will be returned at a later time, but without financial recompense. Non-fungible goods must be loaned out and returned as an individual entities, whereas fungible goods may be returned as a like-for-like replacement."@en ;
    rdfs:isDefinedBy <http://linked.data.gov.au/def/transaction-type> ;
    skos:inScheme <http://linked.data.gov.au/def/transaction-type> ;
    skos:prefLabel "Loan"@en .

trns:borrow a skos:Concept ;
    skos:topConceptOf <http://linked.data.gov.au/def/transaction-type> ;
    skos:definition "The receipt of goods with the agreement that the goods will be returned at a later time, without financial recompense . Non-fungible goods must be borrowed and returned as individual entities, whereas fungible goods may be returned as a like-for-like replacement."@en ;
    rdfs:isDefinedBy <http://linked.data.gov.au/def/transaction-type> ;
    skos:inScheme <http://linked.data.gov.au/def/transaction-type> ;
    skos:prefLabel "Borrow"@en .

trns:exchange a skos:Concept ;
    skos:altLabel "Trade"@en,
        "Swap"@en ;
    skos:topConceptOf <http://linked.data.gov.au/def/transaction-type> ;
    skos:definition "The exchange of goods or services where the value of the transaction is balanced in the form of good-for-goods, goods-for-services, or services-for-services, rather than as a monetary exchange."@en ;
    rdfs:isDefinedBy <http://linked.data.gov.au/def/transaction-type> ;
    skos:inScheme <http://linked.data.gov.au/def/transaction-type> ;
    skos:prefLabel "Exchange"@en .

trns:min-transfer a skos:Collection ;
    skos:prefLabel "Mineral Material Transfers"@en ;
    skos:definition "The transfers of materials cthat may occur between mineral mines, typically between mines operated by the same parent company."@en ;
    skos:member
        trns:transfer-in,
        trns:transfer-out,
        trns:purchase,
        trns:purchase-feed .
